<?xml version="1.0"?>
<rdf:RDF xmlns="http://tw.rpi.edu/web/Courses/Ontologies/2016/OE_8_TeaTeam/"
     xml:base="http://tw.rpi.edu/web/Courses/Ontologies/2016/OE_8_TeaTeam/"
     xmlns:tea="http://tw.rpi.edu/web/Courses/Ontologies/2016/OE_8_TeaTeam/"
     xmlns:np="http://www.nanopub.org/nschema#"
     xmlns:dct="http://purl.org/dc/terms/"
     xmlns:rdf="http://www.w3.org/1999/02/22-rdf-syntax-ns#"
     xmlns:owl="http://www.w3.org/2002/07/owl#"
     xmlns:xml="http://www.w3.org/XML/1998/namespace"
     xmlns:xsd="http://www.w3.org/2001/XMLSchema#"
     xmlns:skos="http://www.w3.org/2004/02/skos/core#"
     xmlns:rdfs="http://www.w3.org/2000/01/rdf-schema#"
     xmlns:rdfg-1="http://www.w3.org/2004/03/trix/rdfg-1/">
    <owl:Ontology rdf:about="http://tw.rpi.edu/web/Courses/Ontologies/2016/OE_8_TeaTeam/">
        <owl:imports rdf:resource="http://www.w3.org/2004/02/skos/core"/>
        <rdfs:label>Tea Ontology</rdfs:label>
        <dct:creator xml:lang="en">Cara Reedy</dct:creator>
        <dct:creator xml:lang="en">Katie Chastain</dct:creator>
    </owl:Ontology>
    


    <!-- 
    ///////////////////////////////////////////////////////////////////////////////////////
    //
    // Annotation properties
    //
    ///////////////////////////////////////////////////////////////////////////////////////
     -->

    


    <!-- http://purl.org/dc/terms/abstract -->

    <owl:AnnotationProperty rdf:about="http://purl.org/dc/terms/abstract"/>
    


    <!-- http://purl.org/dc/terms/contributor -->

    <owl:AnnotationProperty rdf:about="http://purl.org/dc/terms/contributor"/>
    


    <!-- http://purl.org/dc/terms/creator -->

    <owl:AnnotationProperty rdf:about="http://purl.org/dc/terms/creator"/>
    


    <!-- http://purl.org/dc/terms/format -->

    <owl:AnnotationProperty rdf:about="http://purl.org/dc/terms/format"/>
    


    <!-- http://purl.org/dc/terms/hasVersion -->

    <owl:AnnotationProperty rdf:about="http://purl.org/dc/terms/hasVersion"/>
    


    <!-- http://purl.org/dc/terms/identifier -->

    <owl:AnnotationProperty rdf:about="http://purl.org/dc/terms/identifier"/>
    


    <!-- http://purl.org/dc/terms/issued -->

    <owl:AnnotationProperty rdf:about="http://purl.org/dc/terms/issued"/>
    


    <!-- http://purl.org/dc/terms/license -->

    <owl:AnnotationProperty rdf:about="http://purl.org/dc/terms/license"/>
    


    <!-- http://purl.org/dc/terms/references -->

    <owl:AnnotationProperty rdf:about="http://purl.org/dc/terms/references"/>
    


    <!-- http://purl.org/dc/terms/rights -->

    <owl:AnnotationProperty rdf:about="http://purl.org/dc/terms/rights"/>
    


    <!-- http://purl.org/dc/terms/source -->

    <owl:AnnotationProperty rdf:about="http://purl.org/dc/terms/source"/>
    


    <!-- http://purl.org/dc/terms/subject -->

    <owl:AnnotationProperty rdf:about="http://purl.org/dc/terms/subject"/>
    


    <!-- http://purl.org/dc/terms/title -->

    <owl:AnnotationProperty rdf:about="http://purl.org/dc/terms/title"/>
    


    <!-- http://purl.org/dc/terms/type -->

    <owl:AnnotationProperty rdf:about="http://purl.org/dc/terms/type"/>
    


    <!-- http://www.w3.org/2004/02/skos/core#altLabel -->

    <owl:AnnotationProperty rdf:about="http://www.w3.org/2004/02/skos/core#altLabel"/>
    


    <!-- http://www.w3.org/2004/02/skos/core#changeNote -->

    <owl:AnnotationProperty rdf:about="http://www.w3.org/2004/02/skos/core#changeNote"/>
    


    <!-- http://www.w3.org/2004/02/skos/core#definition -->

    <owl:AnnotationProperty rdf:about="http://www.w3.org/2004/02/skos/core#definition"/>
    


    <!-- http://www.w3.org/2004/02/skos/core#editorialNote -->

    <owl:AnnotationProperty rdf:about="http://www.w3.org/2004/02/skos/core#editorialNote"/>
    


    <!-- http://www.w3.org/2004/02/skos/core#example -->

    <owl:AnnotationProperty rdf:about="http://www.w3.org/2004/02/skos/core#example"/>
    


    <!-- http://www.w3.org/2004/02/skos/core#historyNote -->

    <owl:AnnotationProperty rdf:about="http://www.w3.org/2004/02/skos/core#historyNote"/>
    


    <!-- http://www.w3.org/2004/02/skos/core#note -->

    <owl:AnnotationProperty rdf:about="http://www.w3.org/2004/02/skos/core#note"/>
    


    <!-- http://www.w3.org/2004/02/skos/core#prefLabel -->

    <owl:AnnotationProperty rdf:about="http://www.w3.org/2004/02/skos/core#prefLabel"/>
    


    <!-- http://www.w3.org/2004/02/skos/core#scopeNote -->

    <owl:AnnotationProperty rdf:about="http://www.w3.org/2004/02/skos/core#scopeNote"/>
    


    <!-- 
    ///////////////////////////////////////////////////////////////////////////////////////
    //
    // Object Properties
    //
    ///////////////////////////////////////////////////////////////////////////////////////
     -->

    


    <!-- http://tw.rpi.edu/web/Courses/Ontologies/2016/OE_8_TeaTeam/brews -->

    <owl:ObjectProperty rdf:about="http://tw.rpi.edu/web/Courses/Ontologies/2016/OE_8_TeaTeam/brews">
        <owl:inverseOf rdf:resource="http://tw.rpi.edu/web/Courses/Ontologies/2016/OE_8_TeaTeam/hasBrewingTemperature"/>
        <rdfs:domain rdf:resource="http://tw.rpi.edu/web/Courses/Ontologies/2016/OE_8_TeaTeam/BrewingTemperature"/>
        <rdfs:comment>the steepedDrinks a particular brewing temperature range can steep</rdfs:comment>
    </owl:ObjectProperty>
    


    <!-- http://tw.rpi.edu/web/Courses/Ontologies/2016/OE_8_TeaTeam/brewsAt -->

    <owl:ObjectProperty rdf:about="http://tw.rpi.edu/web/Courses/Ontologies/2016/OE_8_TeaTeam/brewsAt">
        <rdfs:comment xml:lang="en">Relates a Plant Part to its appropriate Brewing Temperature(s)</rdfs:comment>
    </owl:ObjectProperty>
    


    <!-- http://tw.rpi.edu/web/Courses/Ontologies/2016/OE_8_TeaTeam/contains -->

    <owl:ObjectProperty rdf:about="http://tw.rpi.edu/web/Courses/Ontologies/2016/OE_8_TeaTeam/contains">
        <rdfs:comment>used for blend to indicate which steepedDrinks are part of that blend</rdfs:comment>
    </owl:ObjectProperty>
    


    <!-- http://tw.rpi.edu/web/Courses/Ontologies/2016/OE_8_TeaTeam/flavorOf -->

    <owl:ObjectProperty rdf:about="http://tw.rpi.edu/web/Courses/Ontologies/2016/OE_8_TeaTeam/flavorOf">
        <owl:inverseOf rdf:resource="http://tw.rpi.edu/web/Courses/Ontologies/2016/OE_8_TeaTeam/hasFlavor"/>
        <rdfs:comment>the steepedDrinks a particular flavor flavors</rdfs:comment>
    </owl:ObjectProperty>
    


    <!-- http://tw.rpi.edu/web/Courses/Ontologies/2016/OE_8_TeaTeam/fromSource -->

    <owl:ObjectProperty rdf:about="http://tw.rpi.edu/web/Courses/Ontologies/2016/OE_8_TeaTeam/fromSource"/>
    


    <!-- http://tw.rpi.edu/web/Courses/Ontologies/2016/OE_8_TeaTeam/hasBrewingTemperature -->

    <owl:ObjectProperty rdf:about="http://tw.rpi.edu/web/Courses/Ontologies/2016/OE_8_TeaTeam/hasBrewingTemperature">
        <rdfs:range rdf:resource="http://tw.rpi.edu/web/Courses/Ontologies/2016/OE_8_TeaTeam/BrewingTemperature"/>
        <owl:propertyChainAxiom rdf:parseType="Collection">
            <rdf:Description rdf:about="http://tw.rpi.edu/web/Courses/Ontologies/2016/OE_8_TeaTeam/madeFromPart"/>
            <rdf:Description rdf:about="http://tw.rpi.edu/web/Courses/Ontologies/2016/OE_8_TeaTeam/brewsAt"/>
        </owl:propertyChainAxiom>
        <rdfs:comment>the brewing temperature range used for a particular steepedDrink</rdfs:comment>
    </owl:ObjectProperty>
    


    <!-- http://tw.rpi.edu/web/Courses/Ontologies/2016/OE_8_TeaTeam/hasCaffeine -->

    <owl:ObjectProperty rdf:about="http://tw.rpi.edu/web/Courses/Ontologies/2016/OE_8_TeaTeam/hasCaffeine">
        <rdfs:range rdf:resource="http://tw.rpi.edu/web/Courses/Ontologies/2016/OE_8_TeaTeam/Caffeination"/>
        <rdfs:comment>has caffeination value of caffeine or no caffeine</rdfs:comment>
    </owl:ObjectProperty>
    


    <!-- http://tw.rpi.edu/web/Courses/Ontologies/2016/OE_8_TeaTeam/hasFlavor -->

    <owl:ObjectProperty rdf:about="http://tw.rpi.edu/web/Courses/Ontologies/2016/OE_8_TeaTeam/hasFlavor">
        <rdfs:comment>the flavor of a particular steepedDrink</rdfs:comment>
    </owl:ObjectProperty>
    


    <!-- http://tw.rpi.edu/web/Courses/Ontologies/2016/OE_8_TeaTeam/madeFromPart -->

    <owl:ObjectProperty rdf:about="http://tw.rpi.edu/web/Courses/Ontologies/2016/OE_8_TeaTeam/madeFromPart">
        <rdfs:range rdf:resource="http://tw.rpi.edu/web/Courses/Ontologies/2016/OE_8_TeaTeam/PlantPart"/>
        <rdfs:comment>defines what kind of plant part a tisane is made from</rdfs:comment>
    </owl:ObjectProperty>
    


    <!-- http://tw.rpi.edu/web/Courses/Ontologies/2016/OE_8_TeaTeam/withStrength -->

    <owl:ObjectProperty rdf:about="http://tw.rpi.edu/web/Courses/Ontologies/2016/OE_8_TeaTeam/withStrength">
        <rdfs:domain rdf:resource="http://tw.rpi.edu/web/Courses/Ontologies/2016/OE_8_TeaTeam/FlavorCompatibility"/>
    </owl:ObjectProperty>
    


    <!-- 
    ///////////////////////////////////////////////////////////////////////////////////////
    //
    // Classes
    //
    ///////////////////////////////////////////////////////////////////////////////////////
     -->

    


    <!-- http://tw.rpi.edu/web/Courses/Ontologies/2016/OE_8_TeaTeam/ASTASpiceFlavor -->

    <owl:Class rdf:about="http://tw.rpi.edu/web/Courses/Ontologies/2016/OE_8_TeaTeam/ASTASpiceFlavor">
        <rdfs:subClassOf rdf:resource="http://tw.rpi.edu/web/Courses/Ontologies/2016/OE_8_TeaTeam/Flavor"/>
        <rdfs:comment>a flavor which comes from a spice defined by the ASTA spice list</rdfs:comment>
        <rdfs:label xml:lang="en">ASTA spice flavor</rdfs:label>
    </owl:Class>
    


    <!-- http://tw.rpi.edu/web/Courses/Ontologies/2016/OE_8_TeaTeam/AgedRipePu-ErhTea -->

    <owl:Class rdf:about="http://tw.rpi.edu/web/Courses/Ontologies/2016/OE_8_TeaTeam/AgedRipePu-ErhTea">
        <rdfs:subClassOf rdf:resource="http://tw.rpi.edu/web/Courses/Ontologies/2016/OE_8_TeaTeam/Pu-ErhTea"/>
        <rdfs:subClassOf>
            <owl:Restriction>
                <owl:onProperty rdf:resource="http://tw.rpi.edu/web/Courses/Ontologies/2016/OE_8_TeaTeam/hasBrewingTemperature"/>
                <owl:someValuesFrom rdf:resource="http://tw.rpi.edu/web/Courses/Ontologies/2016/OE_8_TeaTeam/HighBrewingTemperature"/>
            </owl:Restriction>
        </rdfs:subClassOf>
        <rdfs:comment>A pu-erh tea that is at least three years old</rdfs:comment>
        <rdfs:label xml:lang="en">aged ripe pu-erh tea</rdfs:label>
    </owl:Class>
    


    <!-- http://tw.rpi.edu/web/Courses/Ontologies/2016/OE_8_TeaTeam/AllspiceFlavor -->

    <owl:Class rdf:about="http://tw.rpi.edu/web/Courses/Ontologies/2016/OE_8_TeaTeam/AllspiceFlavor">
        <rdfs:subClassOf rdf:resource="http://tw.rpi.edu/web/Courses/Ontologies/2016/OE_8_TeaTeam/ASTASpiceFlavor"/>
        <rdfs:subClassOf rdf:resource="http://tw.rpi.edu/web/Courses/Ontologies/2016/OE_8_TeaTeam/SpicyFlavor"/>
        <rdfs:comment>a flavor listed in the ASTA list that is reminiscent of allspice, the dried berries of Pimenta dioica</rdfs:comment>
        <rdfs:label xml:lang="en">allspice flavor</rdfs:label>
    </owl:Class>
    


    <!-- http://tw.rpi.edu/web/Courses/Ontologies/2016/OE_8_TeaTeam/AnimalFlavor -->

    <owl:Class rdf:about="http://tw.rpi.edu/web/Courses/Ontologies/2016/OE_8_TeaTeam/AnimalFlavor">
        <rdfs:subClassOf rdf:resource="http://tw.rpi.edu/web/Courses/Ontologies/2016/OE_8_TeaTeam/Flavor"/>
        <rdfs:comment xml:lang="en">a flavor that is musky or evocative of leather</rdfs:comment>
        <rdfs:label xml:lang="en">animal flavor</rdfs:label>
    </owl:Class>
    


    <!-- http://tw.rpi.edu/web/Courses/Ontologies/2016/OE_8_TeaTeam/AniseFlavor -->

    <owl:Class rdf:about="http://tw.rpi.edu/web/Courses/Ontologies/2016/OE_8_TeaTeam/AniseFlavor">
        <rdfs:subClassOf rdf:resource="http://tw.rpi.edu/web/Courses/Ontologies/2016/OE_8_TeaTeam/ASTASpiceFlavor"/>
        <rdfs:subClassOf rdf:resource="http://tw.rpi.edu/web/Courses/Ontologies/2016/OE_8_TeaTeam/SpicyFlavor"/>
        <rdfs:comment>a flavor listed in the ASTA list that is reminiscent of anise, Pimpinella ansium</rdfs:comment>
        <rdfs:label xml:lang="en">anise flavor</rdfs:label>
    </owl:Class>
    


    <!-- http://tw.rpi.edu/web/Courses/Ontologies/2016/OE_8_TeaTeam/ArilPart -->

    <owl:Class rdf:about="http://tw.rpi.edu/web/Courses/Ontologies/2016/OE_8_TeaTeam/ArilPart">
        <rdfs:subClassOf rdf:resource="http://tw.rpi.edu/web/Courses/Ontologies/2016/OE_8_TeaTeam/PlantPart"/>
        <rdfs:subClassOf>
            <owl:Restriction>
                <owl:onProperty rdf:resource="http://tw.rpi.edu/web/Courses/Ontologies/2016/OE_8_TeaTeam/brewsAt"/>
                <owl:someValuesFrom rdf:resource="http://tw.rpi.edu/web/Courses/Ontologies/2016/OE_8_TeaTeam/HighBrewingTemperature"/>
            </owl:Restriction>
        </rdfs:subClassOf>
        <rdfs:subClassOf>
            <owl:Restriction>
                <owl:onProperty rdf:resource="http://tw.rpi.edu/web/Courses/Ontologies/2016/OE_8_TeaTeam/brewsAt"/>
                <owl:someValuesFrom rdf:resource="http://tw.rpi.edu/web/Courses/Ontologies/2016/OE_8_TeaTeam/LowBrewingTemperature"/>
            </owl:Restriction>
        </rdfs:subClassOf>
        <rdfs:subClassOf>
            <owl:Restriction>
                <owl:onProperty rdf:resource="http://tw.rpi.edu/web/Courses/Ontologies/2016/OE_8_TeaTeam/brewsAt"/>
                <owl:someValuesFrom rdf:resource="http://tw.rpi.edu/web/Courses/Ontologies/2016/OE_8_TeaTeam/MediumBrewingTemperature"/>
            </owl:Restriction>
        </rdfs:subClassOf>
        <rdfs:comment>the aril of a plant, a growth that partially or fully covers a seed and may look like a fruit itself</rdfs:comment>
        <rdfs:label xml:lang="en">aril plant part</rdfs:label>
    </owl:Class>
    


    <!-- http://tw.rpi.edu/web/Courses/Ontologies/2016/OE_8_TeaTeam/BanchaGreenTea -->

    <owl:Class rdf:about="http://tw.rpi.edu/web/Courses/Ontologies/2016/OE_8_TeaTeam/BanchaGreenTea">
        <rdfs:subClassOf rdf:resource="http://tw.rpi.edu/web/Courses/Ontologies/2016/OE_8_TeaTeam/GreenTea"/>
        <rdfs:comment>A green tea from Japan produced from unshaded steamed leaves that are picked in summer or autumn</rdfs:comment>
        <rdfs:label xml:lang="en">bancha green tea</rdfs:label>
    </owl:Class>
    


    <!-- http://tw.rpi.edu/web/Courses/Ontologies/2016/OE_8_TeaTeam/BarkPart -->

    <owl:Class rdf:about="http://tw.rpi.edu/web/Courses/Ontologies/2016/OE_8_TeaTeam/BarkPart">
        <rdfs:subClassOf rdf:resource="http://tw.rpi.edu/web/Courses/Ontologies/2016/OE_8_TeaTeam/PlantPart"/>
        <rdfs:subClassOf>
            <owl:Restriction>
                <owl:onProperty rdf:resource="http://tw.rpi.edu/web/Courses/Ontologies/2016/OE_8_TeaTeam/brewsAt"/>
                <owl:someValuesFrom rdf:resource="http://tw.rpi.edu/web/Courses/Ontologies/2016/OE_8_TeaTeam/HighBrewingTemperature"/>
            </owl:Restriction>
        </rdfs:subClassOf>
        <rdfs:comment>the bark of a plant, the tough external covering of the stems or roots of woody plants</rdfs:comment>
        <rdfs:label xml:lang="en">bark part</rdfs:label>
    </owl:Class>
    


    <!-- http://tw.rpi.edu/web/Courses/Ontologies/2016/OE_8_TeaTeam/BasilFlavor -->

    <owl:Class rdf:about="http://tw.rpi.edu/web/Courses/Ontologies/2016/OE_8_TeaTeam/BasilFlavor">
        <rdfs:subClassOf rdf:resource="http://tw.rpi.edu/web/Courses/Ontologies/2016/OE_8_TeaTeam/ASTASpiceFlavor"/>
        <rdfs:comment>a flavor listed in the ASTA list that is reminiscent of basil, the leaves of Ocimum basilicum</rdfs:comment>
        <rdfs:label xml:lang="en">basil flavor</rdfs:label>
    </owl:Class>
    


    <!-- http://tw.rpi.edu/web/Courses/Ontologies/2016/OE_8_TeaTeam/BayLeafFlavor -->

    <owl:Class rdf:about="http://tw.rpi.edu/web/Courses/Ontologies/2016/OE_8_TeaTeam/BayLeafFlavor">
        <rdfs:subClassOf rdf:resource="http://tw.rpi.edu/web/Courses/Ontologies/2016/OE_8_TeaTeam/ASTASpiceFlavor"/>
        <rdfs:subClassOf rdf:resource="http://tw.rpi.edu/web/Courses/Ontologies/2016/OE_8_TeaTeam/HerbalFlavor"/>
        <rdfs:comment>a flavor listed in the ASTA list that is reminiscent of bay leaves, a spice made from the leaves of one of several trees in the Lauraceae or Myrtaceae families</rdfs:comment>
        <rdfs:label xml:lang="en">bay leaf flavor</rdfs:label>
    </owl:Class>
    


    <!-- http://tw.rpi.edu/web/Courses/Ontologies/2016/OE_8_TeaTeam/BerryPart -->

    <owl:Class rdf:about="http://tw.rpi.edu/web/Courses/Ontologies/2016/OE_8_TeaTeam/BerryPart">
        <rdfs:subClassOf rdf:resource="http://tw.rpi.edu/web/Courses/Ontologies/2016/OE_8_TeaTeam/FruitPart"/>
        <rdfs:comment>culinarily, a fruit that is small and does not have a large seed within it, usually juicy</rdfs:comment>
        <rdfs:label xml:lang="en">berry part</rdfs:label>
    </owl:Class>
    


    <!-- http://tw.rpi.edu/web/Courses/Ontologies/2016/OE_8_TeaTeam/BlackCarawayFlavor -->

    <owl:Class rdf:about="http://tw.rpi.edu/web/Courses/Ontologies/2016/OE_8_TeaTeam/BlackCarawayFlavor">
        <rdfs:subClassOf rdf:resource="http://tw.rpi.edu/web/Courses/Ontologies/2016/OE_8_TeaTeam/ASTASpiceFlavor"/>
        <rdfs:subClassOf rdf:resource="http://tw.rpi.edu/web/Courses/Ontologies/2016/OE_8_TeaTeam/SpicyFlavor"/>
        <rdfs:comment xml:lang="en">a flavor listed in the ASTA list that is reminiscent of black caraway, also known as black cumin, the seeds of the planf Nigella sativa</rdfs:comment>
        <rdfs:label xml:lang="en">black caraway flavor</rdfs:label>
    </owl:Class>
    


    <!-- http://tw.rpi.edu/web/Courses/Ontologies/2016/OE_8_TeaTeam/BlackPepperFlavor -->

    <owl:Class rdf:about="http://tw.rpi.edu/web/Courses/Ontologies/2016/OE_8_TeaTeam/BlackPepperFlavor">
        <rdfs:subClassOf rdf:resource="http://tw.rpi.edu/web/Courses/Ontologies/2016/OE_8_TeaTeam/ASTASpiceFlavor"/>
        <rdfs:subClassOf rdf:resource="http://tw.rpi.edu/web/Courses/Ontologies/2016/OE_8_TeaTeam/SpicyFlavor"/>
        <rdfs:comment>a flavor listed in the ASTA list that is reminiscent of black pepper, the dried fruits of the flowering vine Piper nigrum</rdfs:comment>
        <rdfs:label xml:lang="en">black pepper flavor</rdfs:label>
    </owl:Class>
    


    <!-- http://tw.rpi.edu/web/Courses/Ontologies/2016/OE_8_TeaTeam/BlackTea -->

    <owl:Class rdf:about="http://tw.rpi.edu/web/Courses/Ontologies/2016/OE_8_TeaTeam/BlackTea">
        <rdfs:subClassOf rdf:resource="http://tw.rpi.edu/web/Courses/Ontologies/2016/OE_8_TeaTeam/Tea"/>
        <rdfs:comment>Tea that has been withered, rolled, oxidized, and dried; completely oxidized</rdfs:comment>
        <rdfs:label xml:lang="en">black tea</rdfs:label>
    </owl:Class>
    


    <!-- http://tw.rpi.edu/web/Courses/Ontologies/2016/OE_8_TeaTeam/Blend -->

    <owl:Class rdf:about="http://tw.rpi.edu/web/Courses/Ontologies/2016/OE_8_TeaTeam/Blend">
        <owl:equivalentClass>
            <owl:Restriction>
                <owl:onProperty rdf:resource="http://tw.rpi.edu/web/Courses/Ontologies/2016/OE_8_TeaTeam/contains"/>
                <owl:minQualifiedCardinality rdf:datatype="http://www.w3.org/2001/XMLSchema#nonNegativeInteger">2</owl:minQualifiedCardinality>
                <owl:onClass rdf:resource="http://tw.rpi.edu/web/Courses/Ontologies/2016/OE_8_TeaTeam/SteepedDrink"/>
            </owl:Restriction>
        </owl:equivalentClass>
        <rdfs:subClassOf rdf:resource="http://tw.rpi.edu/web/Courses/Ontologies/2016/OE_8_TeaTeam/DomainConcept"/>
        <rdfs:comment>the combination of at least 2 steepedDrinks</rdfs:comment>
        <rdfs:label xml:lang="en">blend</rdfs:label>
    </owl:Class>
    


    <!-- http://tw.rpi.edu/web/Courses/Ontologies/2016/OE_8_TeaTeam/BrewingTemperature -->

    <owl:Class rdf:about="http://tw.rpi.edu/web/Courses/Ontologies/2016/OE_8_TeaTeam/BrewingTemperature">
        <owl:equivalentClass>
            <owl:Class>
                <owl:unionOf rdf:parseType="Collection">
                    <rdf:Description rdf:about="http://tw.rpi.edu/web/Courses/Ontologies/2016/OE_8_TeaTeam/HighBrewingTemperature"/>
                    <rdf:Description rdf:about="http://tw.rpi.edu/web/Courses/Ontologies/2016/OE_8_TeaTeam/LowBrewingTemperature"/>
                    <rdf:Description rdf:about="http://tw.rpi.edu/web/Courses/Ontologies/2016/OE_8_TeaTeam/MediumBrewingTemperature"/>
                </owl:unionOf>
            </owl:Class>
        </owl:equivalentClass>
        <rdfs:subClassOf rdf:resource="http://tw.rpi.edu/web/Courses/Ontologies/2016/OE_8_TeaTeam/ValuePartition"/>
        <rdfs:subClassOf>
            <owl:Restriction>
                <owl:onProperty rdf:resource="http://tw.rpi.edu/web/Courses/Ontologies/2016/OE_8_TeaTeam/brews"/>
                <owl:minQualifiedCardinality rdf:datatype="http://www.w3.org/2001/XMLSchema#nonNegativeInteger">1</owl:minQualifiedCardinality>
                <owl:onClass rdf:resource="http://tw.rpi.edu/web/Courses/Ontologies/2016/OE_8_TeaTeam/SteepedDrink"/>
            </owl:Restriction>
        </rdfs:subClassOf>
        <rdfs:comment>The temperature of the water in which a steeped beverage is steeped</rdfs:comment>
        <rdfs:label xml:lang="en">brewing temperature</rdfs:label>
    </owl:Class>
    


    <!-- http://tw.rpi.edu/web/Courses/Ontologies/2016/OE_8_TeaTeam/BudPart -->

    <owl:Class rdf:about="http://tw.rpi.edu/web/Courses/Ontologies/2016/OE_8_TeaTeam/BudPart">
        <rdfs:subClassOf rdf:resource="http://tw.rpi.edu/web/Courses/Ontologies/2016/OE_8_TeaTeam/FlowerPart"/>
        <rdfs:comment>an underdeveloped flower</rdfs:comment>
        <rdfs:label xml:lang="en">bud part</rdfs:label>
    </owl:Class>
    


    <!-- http://tw.rpi.edu/web/Courses/Ontologies/2016/OE_8_TeaTeam/Caffeinated -->

    <owl:Class rdf:about="http://tw.rpi.edu/web/Courses/Ontologies/2016/OE_8_TeaTeam/Caffeinated">
        <rdfs:subClassOf rdf:resource="http://tw.rpi.edu/web/Courses/Ontologies/2016/OE_8_TeaTeam/Caffeination"/>
        <owl:disjointWith rdf:resource="http://tw.rpi.edu/web/Courses/Ontologies/2016/OE_8_TeaTeam/Decaffeinated"/>
        <rdfs:comment>Containing caffeine</rdfs:comment>
    </owl:Class>
    


    <!-- http://tw.rpi.edu/web/Courses/Ontologies/2016/OE_8_TeaTeam/CaffeinatedSteepedDrink -->

    <owl:Class rdf:about="http://tw.rpi.edu/web/Courses/Ontologies/2016/OE_8_TeaTeam/CaffeinatedSteepedDrink">
        <owl:equivalentClass>
            <owl:Class>
                <owl:intersectionOf rdf:parseType="Collection">
                    <rdf:Description rdf:about="http://tw.rpi.edu/web/Courses/Ontologies/2016/OE_8_TeaTeam/SteepedDrink"/>
                    <owl:Restriction>
                        <owl:onProperty rdf:resource="http://tw.rpi.edu/web/Courses/Ontologies/2016/OE_8_TeaTeam/hasCaffeine"/>
                        <owl:someValuesFrom rdf:resource="http://tw.rpi.edu/web/Courses/Ontologies/2016/OE_8_TeaTeam/Caffeinated"/>
                    </owl:Restriction>
                </owl:intersectionOf>
            </owl:Class>
        </owl:equivalentClass>
        <rdfs:subClassOf rdf:resource="http://tw.rpi.edu/web/Courses/Ontologies/2016/OE_8_TeaTeam/SteepedDrink"/>
        <owl:disjointWith rdf:resource="http://tw.rpi.edu/web/Courses/Ontologies/2016/OE_8_TeaTeam/DecaffeinatedSteepedDrink"/>
        <rdfs:comment>a steeped drink that contains caffeine</rdfs:comment>
        <rdfs:label xml:lang="en">caffeinated steeped drink</rdfs:label>
    </owl:Class>
    


    <!-- http://tw.rpi.edu/web/Courses/Ontologies/2016/OE_8_TeaTeam/Caffeination -->

    <owl:Class rdf:about="http://tw.rpi.edu/web/Courses/Ontologies/2016/OE_8_TeaTeam/Caffeination">
        <owl:equivalentClass>
            <owl:Class>
                <owl:unionOf rdf:parseType="Collection">
                    <rdf:Description rdf:about="http://tw.rpi.edu/web/Courses/Ontologies/2016/OE_8_TeaTeam/Caffeinated"/>
                    <rdf:Description rdf:about="http://tw.rpi.edu/web/Courses/Ontologies/2016/OE_8_TeaTeam/Decaffeinated"/>
                </owl:unionOf>
            </owl:Class>
        </owl:equivalentClass>
        <rdfs:subClassOf rdf:resource="http://tw.rpi.edu/web/Courses/Ontologies/2016/OE_8_TeaTeam/ValuePartition"/>
        <rdfs:comment>Whether a brew has caffeine in it or not</rdfs:comment>
        <rdfs:label xml:lang="en">caffeination</rdfs:label>
    </owl:Class>
    


    <!-- http://tw.rpi.edu/web/Courses/Ontologies/2016/OE_8_TeaTeam/CapsicumsFlavor -->

    <owl:Class rdf:about="http://tw.rpi.edu/web/Courses/Ontologies/2016/OE_8_TeaTeam/CapsicumsFlavor">
        <rdfs:subClassOf rdf:resource="http://tw.rpi.edu/web/Courses/Ontologies/2016/OE_8_TeaTeam/ASTASpiceFlavor"/>
        <rdfs:subClassOf rdf:resource="http://tw.rpi.edu/web/Courses/Ontologies/2016/OE_8_TeaTeam/SpicyFlavor"/>
        <rdfs:comment>a flavor listed in the ASTA list that is reminiscent of capsicums or peppers, the fruit of plants in the genus Capsicum</rdfs:comment>
        <rdfs:label xml:lang="en">capsicums flavor</rdfs:label>
    </owl:Class>
    


    <!-- http://tw.rpi.edu/web/Courses/Ontologies/2016/OE_8_TeaTeam/CarawaySeedFlavor -->

    <owl:Class rdf:about="http://tw.rpi.edu/web/Courses/Ontologies/2016/OE_8_TeaTeam/CarawaySeedFlavor">
        <rdfs:subClassOf rdf:resource="http://tw.rpi.edu/web/Courses/Ontologies/2016/OE_8_TeaTeam/ASTASpiceFlavor"/>
        <rdfs:subClassOf rdf:resource="http://tw.rpi.edu/web/Courses/Ontologies/2016/OE_8_TeaTeam/SpicyFlavor"/>
        <rdfs:comment>a flavor listed in the ASTA list that is reminiscent of caraway, the fruits of the plant Carum carvi</rdfs:comment>
        <rdfs:label xml:lang="en">caraway seed flavor</rdfs:label>
    </owl:Class>
    


    <!-- http://tw.rpi.edu/web/Courses/Ontologies/2016/OE_8_TeaTeam/CardamomFlavor -->

    <owl:Class rdf:about="http://tw.rpi.edu/web/Courses/Ontologies/2016/OE_8_TeaTeam/CardamomFlavor">
        <rdfs:subClassOf rdf:resource="http://tw.rpi.edu/web/Courses/Ontologies/2016/OE_8_TeaTeam/ASTASpiceFlavor"/>
        <rdfs:subClassOf rdf:resource="http://tw.rpi.edu/web/Courses/Ontologies/2016/OE_8_TeaTeam/SpicyFlavor"/>
        <rdfs:comment>a flavor listed in the ASTA list that is reminiscent of cardamom, the seeds of one of several plants in the Elettaria and Amomum genuses</rdfs:comment>
        <rdfs:label xml:lang="en">cardamom flavor</rdfs:label>
    </owl:Class>
    


    <!-- http://tw.rpi.edu/web/Courses/Ontologies/2016/OE_8_TeaTeam/CelerySeedFlavor -->

    <owl:Class rdf:about="http://tw.rpi.edu/web/Courses/Ontologies/2016/OE_8_TeaTeam/CelerySeedFlavor">
        <rdfs:subClassOf rdf:resource="http://tw.rpi.edu/web/Courses/Ontologies/2016/OE_8_TeaTeam/ASTASpiceFlavor"/>
        <rdfs:subClassOf rdf:resource="http://tw.rpi.edu/web/Courses/Ontologies/2016/OE_8_TeaTeam/SpicyFlavor"/>
        <rdfs:comment>a flavor listed in the ASTA list that is reminiscent of celery seed, actually the fruit of the celery plant, Apium graveolens</rdfs:comment>
        <rdfs:label xml:lang="en">celery seed flavor</rdfs:label>
    </owl:Class>
    


    <!-- http://tw.rpi.edu/web/Courses/Ontologies/2016/OE_8_TeaTeam/ChamomileFlavor -->

    <owl:Class rdf:about="http://tw.rpi.edu/web/Courses/Ontologies/2016/OE_8_TeaTeam/ChamomileFlavor">
        <rdfs:subClassOf rdf:resource="http://tw.rpi.edu/web/Courses/Ontologies/2016/OE_8_TeaTeam/ASTASpiceFlavor"/>
        <rdfs:subClassOf rdf:resource="http://tw.rpi.edu/web/Courses/Ontologies/2016/OE_8_TeaTeam/FloralFlavor"/>
        <rdfs:comment>a flavor listed in the ASTA list that is reminiscent of chamomile, made from one of several species in the the family Asteraceae, most commonly Matricaria chamomilla or Chameamelum nobile</rdfs:comment>
        <rdfs:label xml:lang="en">chamomile flavor</rdfs:label>
    </owl:Class>
    


    <!-- http://tw.rpi.edu/web/Courses/Ontologies/2016/OE_8_TeaTeam/ChervilFlavor -->

    <owl:Class rdf:about="http://tw.rpi.edu/web/Courses/Ontologies/2016/OE_8_TeaTeam/ChervilFlavor">
        <rdfs:subClassOf rdf:resource="http://tw.rpi.edu/web/Courses/Ontologies/2016/OE_8_TeaTeam/ASTASpiceFlavor"/>
        <rdfs:subClassOf rdf:resource="http://tw.rpi.edu/web/Courses/Ontologies/2016/OE_8_TeaTeam/HerbalFlavor"/>
        <rdfs:comment>a flavor listed in the ASTA list that is reminiscent of chervil or French parsley, the plant Anthriscus cerefolium</rdfs:comment>
        <rdfs:label xml:lang="en">chervil flavor</rdfs:label>
    </owl:Class>
    


    <!-- http://tw.rpi.edu/web/Courses/Ontologies/2016/OE_8_TeaTeam/ChiveFlavor -->

    <owl:Class rdf:about="http://tw.rpi.edu/web/Courses/Ontologies/2016/OE_8_TeaTeam/ChiveFlavor">
        <rdfs:subClassOf rdf:resource="http://tw.rpi.edu/web/Courses/Ontologies/2016/OE_8_TeaTeam/ASTASpiceFlavor"/>
        <rdfs:subClassOf rdf:resource="http://tw.rpi.edu/web/Courses/Ontologies/2016/OE_8_TeaTeam/HerbalFlavor"/>
        <rdfs:comment>a flavor listed in the ASTA list that is reminiscent of chive, the leaves of the plant Allium schoenoprasum</rdfs:comment>
        <rdfs:label xml:lang="en">chive flavor</rdfs:label>
    </owl:Class>
    


    <!-- http://tw.rpi.edu/web/Courses/Ontologies/2016/OE_8_TeaTeam/CilantroFlavor -->

    <owl:Class rdf:about="http://tw.rpi.edu/web/Courses/Ontologies/2016/OE_8_TeaTeam/CilantroFlavor">
        <rdfs:subClassOf rdf:resource="http://tw.rpi.edu/web/Courses/Ontologies/2016/OE_8_TeaTeam/ASTASpiceFlavor"/>
        <rdfs:subClassOf rdf:resource="http://tw.rpi.edu/web/Courses/Ontologies/2016/OE_8_TeaTeam/HerbalFlavor"/>
        <rdfs:comment>a flavor listed in the ASTA list that is reminiscent of cilantro or coriander, the leaves of the plant Coriandrum sativum</rdfs:comment>
        <rdfs:label xml:lang="en">cilantro flavor</rdfs:label>
    </owl:Class>
    


    <!-- http://tw.rpi.edu/web/Courses/Ontologies/2016/OE_8_TeaTeam/CinnamonFlavor -->

    <owl:Class rdf:about="http://tw.rpi.edu/web/Courses/Ontologies/2016/OE_8_TeaTeam/CinnamonFlavor">
        <rdfs:subClassOf rdf:resource="http://tw.rpi.edu/web/Courses/Ontologies/2016/OE_8_TeaTeam/ASTASpiceFlavor"/>
        <rdfs:subClassOf rdf:resource="http://tw.rpi.edu/web/Courses/Ontologies/2016/OE_8_TeaTeam/SpicyFlavor"/>
        <rdfs:comment>a flavor listed in the ASTA list that is reminiscent of cinnamon, the bark of one of several species in the Cinnamomum genus</rdfs:comment>
        <rdfs:label xml:lang="en">cinnamon flavor</rdfs:label>
    </owl:Class>
    


    <!-- http://tw.rpi.edu/web/Courses/Ontologies/2016/OE_8_TeaTeam/CloveFlavor -->

    <owl:Class rdf:about="http://tw.rpi.edu/web/Courses/Ontologies/2016/OE_8_TeaTeam/CloveFlavor">
        <rdfs:subClassOf rdf:resource="http://tw.rpi.edu/web/Courses/Ontologies/2016/OE_8_TeaTeam/ASTASpiceFlavor"/>
        <rdfs:subClassOf rdf:resource="http://tw.rpi.edu/web/Courses/Ontologies/2016/OE_8_TeaTeam/SpicyFlavor"/>
        <rdfs:comment>a flavor listed in the ASTA list that is reminiscent of clove, the flower buds of the tree Syzygium aromaticum</rdfs:comment>
        <rdfs:label xml:lang="en">clove flavor</rdfs:label>
    </owl:Class>
    


    <!-- http://tw.rpi.edu/web/Courses/Ontologies/2016/OE_8_TeaTeam/CompatibleBlend -->

    <owl:Class rdf:about="http://tw.rpi.edu/web/Courses/Ontologies/2016/OE_8_TeaTeam/CompatibleBlend">
        <owl:equivalentClass>
            <owl:Restriction>
                <owl:onProperty rdf:resource="http://tw.rpi.edu/web/Courses/Ontologies/2016/OE_8_TeaTeam/contains"/>
                <owl:someValuesFrom rdf:resource="http://tw.rpi.edu/web/Courses/Ontologies/2016/OE_8_TeaTeam/FlavorCompatibility"/>
            </owl:Restriction>
        </owl:equivalentClass>
        <rdfs:subClassOf rdf:resource="http://tw.rpi.edu/web/Courses/Ontologies/2016/OE_8_TeaTeam/Blend"/>
        <rdfs:comment>a blend of at least two drinks whose flavors are considered compatible</rdfs:comment>
        <rdfs:label xml:lang="en">compatible blend</rdfs:label>
    </owl:Class>
    


    <!-- http://tw.rpi.edu/web/Courses/Ontologies/2016/OE_8_TeaTeam/CorianderSeedFlavor -->

    <owl:Class rdf:about="http://tw.rpi.edu/web/Courses/Ontologies/2016/OE_8_TeaTeam/CorianderSeedFlavor">
        <rdfs:subClassOf rdf:resource="http://tw.rpi.edu/web/Courses/Ontologies/2016/OE_8_TeaTeam/ASTASpiceFlavor"/>
        <rdfs:subClassOf rdf:resource="http://tw.rpi.edu/web/Courses/Ontologies/2016/OE_8_TeaTeam/SpicyFlavor"/>
        <rdfs:comment>a flavor listed in the ASTA list that is reminiscent of coriander seed, actually the fruits of the plant Coriandrum sativum</rdfs:comment>
        <rdfs:label xml:lang="en">coriander flavor</rdfs:label>
    </owl:Class>
    


    <!-- http://tw.rpi.edu/web/Courses/Ontologies/2016/OE_8_TeaTeam/CuminSeedFlavor -->

    <owl:Class rdf:about="http://tw.rpi.edu/web/Courses/Ontologies/2016/OE_8_TeaTeam/CuminSeedFlavor">
        <rdfs:subClassOf rdf:resource="http://tw.rpi.edu/web/Courses/Ontologies/2016/OE_8_TeaTeam/ASTASpiceFlavor"/>
        <rdfs:subClassOf rdf:resource="http://tw.rpi.edu/web/Courses/Ontologies/2016/OE_8_TeaTeam/SpicyFlavor"/>
        <rdfs:comment>a flavor listed in the ASTA list that is reminiscent of cumin, the seeds of the plant Cuminum cyminum</rdfs:comment>
        <rdfs:label xml:lang="en">cumin seed flavor</rdfs:label>
    </owl:Class>
    


    <!-- http://tw.rpi.edu/web/Courses/Ontologies/2016/OE_8_TeaTeam/Decaffeinated -->

    <owl:Class rdf:about="http://tw.rpi.edu/web/Courses/Ontologies/2016/OE_8_TeaTeam/Decaffeinated">
        <rdfs:subClassOf rdf:resource="http://tw.rpi.edu/web/Courses/Ontologies/2016/OE_8_TeaTeam/Caffeination"/>
        <rdfs:comment>Not containing caffeine</rdfs:comment>
    </owl:Class>
    


    <!-- http://tw.rpi.edu/web/Courses/Ontologies/2016/OE_8_TeaTeam/DecaffeinatedBlend -->

    <owl:Class rdf:about="http://tw.rpi.edu/web/Courses/Ontologies/2016/OE_8_TeaTeam/DecaffeinatedBlend">
        <owl:equivalentClass>
            <owl:Restriction>
                <owl:onProperty rdf:resource="http://tw.rpi.edu/web/Courses/Ontologies/2016/OE_8_TeaTeam/contains"/>
                <owl:allValuesFrom rdf:resource="http://tw.rpi.edu/web/Courses/Ontologies/2016/OE_8_TeaTeam/DecaffeinatedSteepedDrink"/>
            </owl:Restriction>
        </owl:equivalentClass>
        <rdfs:subClassOf rdf:resource="http://tw.rpi.edu/web/Courses/Ontologies/2016/OE_8_TeaTeam/Blend"/>
        <rdfs:comment>a blend which does not contain any steeped drinks that contain caffeine</rdfs:comment>
        <rdfs:label xml:lang="en">decaffeinated blend</rdfs:label>
    </owl:Class>
    


    <!-- http://tw.rpi.edu/web/Courses/Ontologies/2016/OE_8_TeaTeam/DecaffeinatedSteepedDrink -->

    <owl:Class rdf:about="http://tw.rpi.edu/web/Courses/Ontologies/2016/OE_8_TeaTeam/DecaffeinatedSteepedDrink">
        <owl:equivalentClass>
            <owl:Class>
                <owl:intersectionOf rdf:parseType="Collection">
                    <rdf:Description rdf:about="http://tw.rpi.edu/web/Courses/Ontologies/2016/OE_8_TeaTeam/SteepedDrink"/>
                    <owl:Restriction>
                        <owl:onProperty rdf:resource="http://tw.rpi.edu/web/Courses/Ontologies/2016/OE_8_TeaTeam/hasCaffeine"/>
                        <owl:allValuesFrom rdf:resource="http://tw.rpi.edu/web/Courses/Ontologies/2016/OE_8_TeaTeam/Decaffeinated"/>
                    </owl:Restriction>
                </owl:intersectionOf>
            </owl:Class>
        </owl:equivalentClass>
        <rdfs:subClassOf rdf:resource="http://tw.rpi.edu/web/Courses/Ontologies/2016/OE_8_TeaTeam/SteepedDrink"/>
        <rdfs:comment>a steeped drink which does not contain caffeine</rdfs:comment>
        <rdfs:label xml:lang="en">decaffeinated steeped drink</rdfs:label>
    </owl:Class>
    


    <!-- http://tw.rpi.edu/web/Courses/Ontologies/2016/OE_8_TeaTeam/DillSeedFlavor -->

    <owl:Class rdf:about="http://tw.rpi.edu/web/Courses/Ontologies/2016/OE_8_TeaTeam/DillSeedFlavor">
        <rdfs:subClassOf rdf:resource="http://tw.rpi.edu/web/Courses/Ontologies/2016/OE_8_TeaTeam/ASTASpiceFlavor"/>
        <rdfs:subClassOf rdf:resource="http://tw.rpi.edu/web/Courses/Ontologies/2016/OE_8_TeaTeam/SpicyFlavor"/>
        <rdfs:comment>a flavor listed in the ASTA list that is reminiscent of dill seed, the seed of the plant Anethum graveolens</rdfs:comment>
        <rdfs:label xml:lang="en">dill seed flavor</rdfs:label>
    </owl:Class>
    


    <!-- http://tw.rpi.edu/web/Courses/Ontologies/2016/OE_8_TeaTeam/DillWeedFlavor -->

    <owl:Class rdf:about="http://tw.rpi.edu/web/Courses/Ontologies/2016/OE_8_TeaTeam/DillWeedFlavor">
        <rdfs:subClassOf rdf:resource="http://tw.rpi.edu/web/Courses/Ontologies/2016/OE_8_TeaTeam/ASTASpiceFlavor"/>
        <rdfs:subClassOf rdf:resource="http://tw.rpi.edu/web/Courses/Ontologies/2016/OE_8_TeaTeam/HerbalFlavor"/>
        <rdfs:comment>a flavor listed in the ASTA list that is reminiscent of dill weed, the leaves of the plant Anethum graveolens</rdfs:comment>
        <rdfs:label xml:lang="en">dill weed flavor</rdfs:label>
    </owl:Class>
    


    <!-- http://tw.rpi.edu/web/Courses/Ontologies/2016/OE_8_TeaTeam/DomainConcept -->

    <owl:Class rdf:about="http://tw.rpi.edu/web/Courses/Ontologies/2016/OE_8_TeaTeam/DomainConcept">
        <owl:disjointWith rdf:resource="http://tw.rpi.edu/web/Courses/Ontologies/2016/OE_8_TeaTeam/ValuePartition"/>
        <rdfs:label xml:lang="en">domain concept</rdfs:label>
    </owl:Class>
    


    <!-- http://tw.rpi.edu/web/Courses/Ontologies/2016/OE_8_TeaTeam/EarthyFlavor -->

    <owl:Class rdf:about="http://tw.rpi.edu/web/Courses/Ontologies/2016/OE_8_TeaTeam/EarthyFlavor">
        <rdfs:subClassOf rdf:resource="http://tw.rpi.edu/web/Courses/Ontologies/2016/OE_8_TeaTeam/Flavor"/>
        <rdfs:comment xml:lang="en">a flavor that is peaty or evocative of dirt or soil</rdfs:comment>
        <rdfs:label xml:lang="en">earthy flavor</rdfs:label>
    </owl:Class>
    


    <!-- http://tw.rpi.edu/web/Courses/Ontologies/2016/OE_8_TeaTeam/FennelSeedFlavor -->

    <owl:Class rdf:about="http://tw.rpi.edu/web/Courses/Ontologies/2016/OE_8_TeaTeam/FennelSeedFlavor">
        <rdfs:subClassOf rdf:resource="http://tw.rpi.edu/web/Courses/Ontologies/2016/OE_8_TeaTeam/ASTASpiceFlavor"/>
        <rdfs:subClassOf rdf:resource="http://tw.rpi.edu/web/Courses/Ontologies/2016/OE_8_TeaTeam/SpicyFlavor"/>
        <rdfs:comment>a flavor listed in the ASTA list that is reminiscent of fennel, the seed of the flowering plant Foeniculum vulgare</rdfs:comment>
        <rdfs:label xml:lang="en">fennel seed flavor</rdfs:label>
    </owl:Class>
    


    <!-- http://tw.rpi.edu/web/Courses/Ontologies/2016/OE_8_TeaTeam/FenugreekSeedFlavor -->

    <owl:Class rdf:about="http://tw.rpi.edu/web/Courses/Ontologies/2016/OE_8_TeaTeam/FenugreekSeedFlavor">
        <rdfs:subClassOf rdf:resource="http://tw.rpi.edu/web/Courses/Ontologies/2016/OE_8_TeaTeam/ASTASpiceFlavor"/>
        <rdfs:subClassOf rdf:resource="http://tw.rpi.edu/web/Courses/Ontologies/2016/OE_8_TeaTeam/SpicyFlavor"/>
        <rdfs:comment>a flavor listed in the ASTA list that is reminiscent of fenugreek, the seeds of the plant Trigonella foenum-graecum</rdfs:comment>
        <rdfs:label xml:lang="en">fenugreek seed flavor</rdfs:label>
    </owl:Class>
    


    <!-- http://tw.rpi.edu/web/Courses/Ontologies/2016/OE_8_TeaTeam/Flavor -->

    <owl:Class rdf:about="http://tw.rpi.edu/web/Courses/Ontologies/2016/OE_8_TeaTeam/Flavor">
        <rdfs:subClassOf rdf:resource="http://tw.rpi.edu/web/Courses/Ontologies/2016/OE_8_TeaTeam/DomainConcept"/>
        <rdfs:comment xml:lang="en">the blend of taste and smell sensations evoked by a substance in the mouth</rdfs:comment>
        <rdfs:isDefinedBy xml:lang="en">Merriam-Webster online dictionary</rdfs:isDefinedBy>
        <rdfs:label xml:lang="en">flavor</rdfs:label>
    </owl:Class>
    


    <!-- http://tw.rpi.edu/web/Courses/Ontologies/2016/OE_8_TeaTeam/FlavorCompatibility -->

    <owl:Class rdf:about="http://tw.rpi.edu/web/Courses/Ontologies/2016/OE_8_TeaTeam/FlavorCompatibility">
        <rdfs:subClassOf rdf:resource="http://tw.rpi.edu/web/Courses/Ontologies/2016/OE_8_TeaTeam/DomainConcept"/>
        <rdfs:comment xml:lang="en">Two or more flavors deemed to be compatible by some source with some strength</rdfs:comment>
        <rdfs:label xml:lang="en">flavor compatibility</rdfs:label>
    </owl:Class>
    


    <!-- http://tw.rpi.edu/web/Courses/Ontologies/2016/OE_8_TeaTeam/FloralFlavor -->

    <owl:Class rdf:about="http://tw.rpi.edu/web/Courses/Ontologies/2016/OE_8_TeaTeam/FloralFlavor">
        <rdfs:subClassOf rdf:resource="http://tw.rpi.edu/web/Courses/Ontologies/2016/OE_8_TeaTeam/Flavor"/>
        <rdfs:comment xml:lang="en">a flavor that is evocative of flowers</rdfs:comment>
        <rdfs:label xml:lang="en">floral flavor</rdfs:label>
    </owl:Class>
    


    <!-- http://tw.rpi.edu/web/Courses/Ontologies/2016/OE_8_TeaTeam/FlowerPart -->

    <owl:Class rdf:about="http://tw.rpi.edu/web/Courses/Ontologies/2016/OE_8_TeaTeam/FlowerPart">
        <rdfs:subClassOf rdf:resource="http://tw.rpi.edu/web/Courses/Ontologies/2016/OE_8_TeaTeam/PlantPart"/>
        <rdfs:subClassOf>
            <owl:Restriction>
                <owl:onProperty rdf:resource="http://tw.rpi.edu/web/Courses/Ontologies/2016/OE_8_TeaTeam/brewsAt"/>
                <owl:someValuesFrom rdf:resource="http://tw.rpi.edu/web/Courses/Ontologies/2016/OE_8_TeaTeam/HighBrewingTemperature"/>
            </owl:Restriction>
        </rdfs:subClassOf>
        <rdfs:subClassOf>
            <owl:Restriction>
                <owl:onProperty rdf:resource="http://tw.rpi.edu/web/Courses/Ontologies/2016/OE_8_TeaTeam/brewsAt"/>
                <owl:someValuesFrom rdf:resource="http://tw.rpi.edu/web/Courses/Ontologies/2016/OE_8_TeaTeam/LowBrewingTemperature"/>
            </owl:Restriction>
        </rdfs:subClassOf>
        <rdfs:subClassOf>
            <owl:Restriction>
                <owl:onProperty rdf:resource="http://tw.rpi.edu/web/Courses/Ontologies/2016/OE_8_TeaTeam/brewsAt"/>
                <owl:someValuesFrom rdf:resource="http://tw.rpi.edu/web/Courses/Ontologies/2016/OE_8_TeaTeam/MediumBrewingTemperature"/>
            </owl:Restriction>
        </rdfs:subClassOf>
        <rdfs:comment>the flower of a plant, the reproductive structure of flowering plants</rdfs:comment>
        <rdfs:label xml:lang="en">flower part</rdfs:label>
    </owl:Class>
    


    <!-- http://tw.rpi.edu/web/Courses/Ontologies/2016/OE_8_TeaTeam/FruitPart -->

    <owl:Class rdf:about="http://tw.rpi.edu/web/Courses/Ontologies/2016/OE_8_TeaTeam/FruitPart">
        <rdfs:subClassOf rdf:resource="http://tw.rpi.edu/web/Courses/Ontologies/2016/OE_8_TeaTeam/PlantPart"/>
        <rdfs:subClassOf>
            <owl:Restriction>
                <owl:onProperty rdf:resource="http://tw.rpi.edu/web/Courses/Ontologies/2016/OE_8_TeaTeam/brewsAt"/>
                <owl:someValuesFrom rdf:resource="http://tw.rpi.edu/web/Courses/Ontologies/2016/OE_8_TeaTeam/HighBrewingTemperature"/>
            </owl:Restriction>
        </rdfs:subClassOf>
        <rdfs:comment>the developed ovary of flowering plants</rdfs:comment>
        <rdfs:label xml:lang="en">fruit part</rdfs:label>
    </owl:Class>
    


    <!-- http://tw.rpi.edu/web/Courses/Ontologies/2016/OE_8_TeaTeam/FruityFlavor -->

    <owl:Class rdf:about="http://tw.rpi.edu/web/Courses/Ontologies/2016/OE_8_TeaTeam/FruityFlavor">
        <rdfs:subClassOf rdf:resource="http://tw.rpi.edu/web/Courses/Ontologies/2016/OE_8_TeaTeam/Flavor"/>
        <rdfs:comment xml:lang="en">a flavor that is evocative of fruit</rdfs:comment>
        <rdfs:label xml:lang="en">fruity flavor</rdfs:label>
    </owl:Class>
    


    <!-- http://tw.rpi.edu/web/Courses/Ontologies/2016/OE_8_TeaTeam/GalangalFlavor -->

    <owl:Class rdf:about="http://tw.rpi.edu/web/Courses/Ontologies/2016/OE_8_TeaTeam/GalangalFlavor">
        <rdfs:subClassOf rdf:resource="http://tw.rpi.edu/web/Courses/Ontologies/2016/OE_8_TeaTeam/ASTASpiceFlavor"/>
        <rdfs:subClassOf rdf:resource="http://tw.rpi.edu/web/Courses/Ontologies/2016/OE_8_TeaTeam/SpicyFlavor"/>
        <rdfs:comment>a flavor listed in the ASTA list that is reminiscent of galangal, the rhizome of one of several plants in the Zingiberaceae family</rdfs:comment>
        <rdfs:label xml:lang="en">galangal flavor</rdfs:label>
    </owl:Class>
    


    <!-- http://tw.rpi.edu/web/Courses/Ontologies/2016/OE_8_TeaTeam/GingerFlavor -->

    <owl:Class rdf:about="http://tw.rpi.edu/web/Courses/Ontologies/2016/OE_8_TeaTeam/GingerFlavor">
        <rdfs:subClassOf rdf:resource="http://tw.rpi.edu/web/Courses/Ontologies/2016/OE_8_TeaTeam/ASTASpiceFlavor"/>
        <rdfs:subClassOf rdf:resource="http://tw.rpi.edu/web/Courses/Ontologies/2016/OE_8_TeaTeam/SpicyFlavor"/>
        <rdfs:comment>a flavor listed in the ASTA list that is reminiscent of ginger, the rhizome of the flowering plant Zingiber officinale</rdfs:comment>
        <rdfs:label xml:lang="en">ginger flavor</rdfs:label>
    </owl:Class>
    


    <!-- http://tw.rpi.edu/web/Courses/Ontologies/2016/OE_8_TeaTeam/GreenPeppercornFlavor -->

    <owl:Class rdf:about="http://tw.rpi.edu/web/Courses/Ontologies/2016/OE_8_TeaTeam/GreenPeppercornFlavor">
        <rdfs:subClassOf rdf:resource="http://tw.rpi.edu/web/Courses/Ontologies/2016/OE_8_TeaTeam/ASTASpiceFlavor"/>
        <rdfs:subClassOf rdf:resource="http://tw.rpi.edu/web/Courses/Ontologies/2016/OE_8_TeaTeam/SpicyFlavor"/>
        <rdfs:comment>a flavor listed in the ASTA list that is reminiscent of green pepper, the unripened seeds of the plant Piper nigrum that have been processed in a way that preserves their green color</rdfs:comment>
        <rdfs:label xml:lang="en">green peppercorn flavor</rdfs:label>
    </owl:Class>
    


    <!-- http://tw.rpi.edu/web/Courses/Ontologies/2016/OE_8_TeaTeam/GreenTea -->

    <owl:Class rdf:about="http://tw.rpi.edu/web/Courses/Ontologies/2016/OE_8_TeaTeam/GreenTea">
        <rdfs:subClassOf rdf:resource="http://tw.rpi.edu/web/Courses/Ontologies/2016/OE_8_TeaTeam/Tea"/>
        <rdfs:subClassOf>
            <owl:Restriction>
                <owl:onProperty rdf:resource="http://tw.rpi.edu/web/Courses/Ontologies/2016/OE_8_TeaTeam/hasBrewingTemperature"/>
                <owl:someValuesFrom rdf:resource="http://tw.rpi.edu/web/Courses/Ontologies/2016/OE_8_TeaTeam/LowBrewingTemperature"/>
            </owl:Restriction>
        </rdfs:subClassOf>
        <rdfs:comment>Tea that has been withered, rolled, and dried, but is not oxidized</rdfs:comment>
        <rdfs:label xml:lang="en">green tea</rdfs:label>
    </owl:Class>
    


    <!-- http://tw.rpi.edu/web/Courses/Ontologies/2016/OE_8_TeaTeam/Guayusa -->

    <owl:Class rdf:about="http://tw.rpi.edu/web/Courses/Ontologies/2016/OE_8_TeaTeam/Guayusa">
        <rdfs:subClassOf rdf:resource="http://tw.rpi.edu/web/Courses/Ontologies/2016/OE_8_TeaTeam/CaffeinatedSteepedDrink"/>
        <rdfs:subClassOf rdf:resource="http://tw.rpi.edu/web/Courses/Ontologies/2016/OE_8_TeaTeam/Tisane"/>
        <rdfs:comment>A steeped drink made from the leaves of Ilex guayusa, grown in South America. Contains caffeine.</rdfs:comment>
        <rdfs:label xml:lang="en">guayusa</rdfs:label>
    </owl:Class>
    


    <!-- http://tw.rpi.edu/web/Courses/Ontologies/2016/OE_8_TeaTeam/GyokurochaGreenTea -->

    <owl:Class rdf:about="http://tw.rpi.edu/web/Courses/Ontologies/2016/OE_8_TeaTeam/GyokurochaGreenTea">
        <rdfs:subClassOf rdf:resource="http://tw.rpi.edu/web/Courses/Ontologies/2016/OE_8_TeaTeam/GreenTea"/>
        <rdfs:comment>A green tea from Japan produced from steamed leaves that were shaded during growth</rdfs:comment>
        <rdfs:label xml:lang="en">gyokurocha green tea</rdfs:label>
    </owl:Class>
    


    <!-- http://tw.rpi.edu/web/Courses/Ontologies/2016/OE_8_TeaTeam/HerbalFlavor -->

    <owl:Class rdf:about="http://tw.rpi.edu/web/Courses/Ontologies/2016/OE_8_TeaTeam/HerbalFlavor">
        <rdfs:subClassOf rdf:resource="http://tw.rpi.edu/web/Courses/Ontologies/2016/OE_8_TeaTeam/Flavor"/>
        <rdfs:comment xml:lang="en">a flavor that is evocative of culinary/medicinal herbs - leaves of plants used for savory or medicinal purposes</rdfs:comment>
        <rdfs:label xml:lang="en">herbal flavor</rdfs:label>
    </owl:Class>
    


    <!-- http://tw.rpi.edu/web/Courses/Ontologies/2016/OE_8_TeaTeam/HighBrewingTemperature -->

    <owl:Class rdf:about="http://tw.rpi.edu/web/Courses/Ontologies/2016/OE_8_TeaTeam/HighBrewingTemperature">
        <rdfs:subClassOf rdf:resource="http://tw.rpi.edu/web/Courses/Ontologies/2016/OE_8_TeaTeam/BrewingTemperature"/>
        <owl:disjointWith rdf:resource="http://tw.rpi.edu/web/Courses/Ontologies/2016/OE_8_TeaTeam/LowBrewingTemperature"/>
        <owl:disjointWith rdf:resource="http://tw.rpi.edu/web/Courses/Ontologies/2016/OE_8_TeaTeam/MediumBrewingTemperature"/>
        <rdfs:comment>205~212°F or 96~100°C</rdfs:comment>
        <rdfs:label xml:lang="en">high brewing temperature</rdfs:label>
    </owl:Class>
    


    <!-- http://tw.rpi.edu/web/Courses/Ontologies/2016/OE_8_TeaTeam/HorseradishFlavor -->

    <owl:Class rdf:about="http://tw.rpi.edu/web/Courses/Ontologies/2016/OE_8_TeaTeam/HorseradishFlavor">
        <rdfs:subClassOf rdf:resource="http://tw.rpi.edu/web/Courses/Ontologies/2016/OE_8_TeaTeam/ASTASpiceFlavor"/>
        <rdfs:subClassOf rdf:resource="http://tw.rpi.edu/web/Courses/Ontologies/2016/OE_8_TeaTeam/SpicyFlavor"/>
        <rdfs:comment>a flavor listed in the ASTA list that is reminiscent of horseradish, the root of the plant Armoracia rusticana</rdfs:comment>
        <rdfs:label xml:lang="en">horseradish flavor</rdfs:label>
    </owl:Class>
    


    <!-- http://tw.rpi.edu/web/Courses/Ontologies/2016/OE_8_TeaTeam/HoujichaGreenTea -->

    <owl:Class rdf:about="http://tw.rpi.edu/web/Courses/Ontologies/2016/OE_8_TeaTeam/HoujichaGreenTea">
        <rdfs:subClassOf rdf:resource="http://tw.rpi.edu/web/Courses/Ontologies/2016/OE_8_TeaTeam/GreenTea"/>
        <rdfs:comment>A green tea from Japan produced from unshaded leaves that are roasted rather than steamed</rdfs:comment>
        <rdfs:label xml:lang="en">houjicha green tea</rdfs:label>
    </owl:Class>
    


    <!-- http://tw.rpi.edu/web/Courses/Ontologies/2016/OE_8_TeaTeam/JuniperFlavor -->

    <owl:Class rdf:about="http://tw.rpi.edu/web/Courses/Ontologies/2016/OE_8_TeaTeam/JuniperFlavor">
        <rdfs:subClassOf rdf:resource="http://tw.rpi.edu/web/Courses/Ontologies/2016/OE_8_TeaTeam/ASTASpiceFlavor"/>
        <rdfs:subClassOf rdf:resource="http://tw.rpi.edu/web/Courses/Ontologies/2016/OE_8_TeaTeam/SpicyFlavor"/>
        <rdfs:comment>a flavor listed in the ASTA list that is reminiscent of juniper berries, from the trees in the genus Juniperus</rdfs:comment>
        <rdfs:label xml:lang="en">juniper flavor</rdfs:label>
    </owl:Class>
    


    <!-- http://tw.rpi.edu/web/Courses/Ontologies/2016/OE_8_TeaTeam/KabusechaGreenTea -->

    <owl:Class rdf:about="http://tw.rpi.edu/web/Courses/Ontologies/2016/OE_8_TeaTeam/KabusechaGreenTea">
        <rdfs:subClassOf rdf:resource="http://tw.rpi.edu/web/Courses/Ontologies/2016/OE_8_TeaTeam/GreenTea"/>
        <rdfs:comment>A green tea from Japan produced from steamed leaves that were shaded during part of the last part of growth before harvest</rdfs:comment>
        <rdfs:label xml:lang="en">kabusecha green tea</rdfs:label>
    </owl:Class>
    


    <!-- http://tw.rpi.edu/web/Courses/Ontologies/2016/OE_8_TeaTeam/LavenderFlavor -->

    <owl:Class rdf:about="http://tw.rpi.edu/web/Courses/Ontologies/2016/OE_8_TeaTeam/LavenderFlavor">
        <rdfs:subClassOf rdf:resource="http://tw.rpi.edu/web/Courses/Ontologies/2016/OE_8_TeaTeam/ASTASpiceFlavor"/>
        <rdfs:subClassOf rdf:resource="http://tw.rpi.edu/web/Courses/Ontologies/2016/OE_8_TeaTeam/FloralFlavor"/>
        <rdfs:comment>a flavor listed in the ASTA list that is reminiscent of lavender, the flowers of the plant Lavandula angustifolia</rdfs:comment>
        <rdfs:label xml:lang="en">lavender flavor</rdfs:label>
    </owl:Class>
    


    <!-- http://tw.rpi.edu/web/Courses/Ontologies/2016/OE_8_TeaTeam/LeafPart -->

    <owl:Class rdf:about="http://tw.rpi.edu/web/Courses/Ontologies/2016/OE_8_TeaTeam/LeafPart">
        <rdfs:subClassOf rdf:resource="http://tw.rpi.edu/web/Courses/Ontologies/2016/OE_8_TeaTeam/PlantPart"/>
        <rdfs:subClassOf>
            <owl:Restriction>
                <owl:onProperty rdf:resource="http://tw.rpi.edu/web/Courses/Ontologies/2016/OE_8_TeaTeam/brewsAt"/>
                <owl:someValuesFrom rdf:resource="http://tw.rpi.edu/web/Courses/Ontologies/2016/OE_8_TeaTeam/HighBrewingTemperature"/>
            </owl:Restriction>
        </rdfs:subClassOf>
        <rdfs:subClassOf>
            <owl:Restriction>
                <owl:onProperty rdf:resource="http://tw.rpi.edu/web/Courses/Ontologies/2016/OE_8_TeaTeam/brewsAt"/>
                <owl:someValuesFrom rdf:resource="http://tw.rpi.edu/web/Courses/Ontologies/2016/OE_8_TeaTeam/LowBrewingTemperature"/>
            </owl:Restriction>
        </rdfs:subClassOf>
        <rdfs:subClassOf>
            <owl:Restriction>
                <owl:onProperty rdf:resource="http://tw.rpi.edu/web/Courses/Ontologies/2016/OE_8_TeaTeam/brewsAt"/>
                <owl:someValuesFrom rdf:resource="http://tw.rpi.edu/web/Courses/Ontologies/2016/OE_8_TeaTeam/MediumBrewingTemperature"/>
            </owl:Restriction>
        </rdfs:subClassOf>
        <rdfs:comment>the structure used by a plant to perform photosynthesis</rdfs:comment>
        <rdfs:label xml:lang="en">leaf part</rdfs:label>
    </owl:Class>
    


    <!-- http://tw.rpi.edu/web/Courses/Ontologies/2016/OE_8_TeaTeam/LemonBalmFlavor -->

    <owl:Class rdf:about="http://tw.rpi.edu/web/Courses/Ontologies/2016/OE_8_TeaTeam/LemonBalmFlavor">
        <rdfs:subClassOf rdf:resource="http://tw.rpi.edu/web/Courses/Ontologies/2016/OE_8_TeaTeam/ASTASpiceFlavor"/>
        <rdfs:subClassOf rdf:resource="http://tw.rpi.edu/web/Courses/Ontologies/2016/OE_8_TeaTeam/HerbalFlavor"/>
        <rdfs:comment>a flavor listed in the ASTA list that is reminiscent of lemon balm, the leaves of the plant Melissa officinalis</rdfs:comment>
        <rdfs:label xml:lang="en">lemon balm flavor</rdfs:label>
    </owl:Class>
    


    <!-- http://tw.rpi.edu/web/Courses/Ontologies/2016/OE_8_TeaTeam/LowBrewingTemperature -->

    <owl:Class rdf:about="http://tw.rpi.edu/web/Courses/Ontologies/2016/OE_8_TeaTeam/LowBrewingTemperature">
        <rdfs:subClassOf rdf:resource="http://tw.rpi.edu/web/Courses/Ontologies/2016/OE_8_TeaTeam/BrewingTemperature"/>
        <owl:disjointWith rdf:resource="http://tw.rpi.edu/web/Courses/Ontologies/2016/OE_8_TeaTeam/MediumBrewingTemperature"/>
        <rdfs:comment>160~185°F or 71~85°C</rdfs:comment>
        <rdfs:label xml:lang="en">low brewing temperature</rdfs:label>
    </owl:Class>
    


    <!-- http://tw.rpi.edu/web/Courses/Ontologies/2016/OE_8_TeaTeam/MacchaGreenTea -->

    <owl:Class rdf:about="http://tw.rpi.edu/web/Courses/Ontologies/2016/OE_8_TeaTeam/MacchaGreenTea">
        <rdfs:subClassOf rdf:resource="http://tw.rpi.edu/web/Courses/Ontologies/2016/OE_8_TeaTeam/GreenTea"/>
        <rdfs:comment>A green tea from Japan produced from steamed leaves that were shaded during growth, then powdered after drying.</rdfs:comment>
        <rdfs:label xml:lang="en">maccha green tea</rdfs:label>
    </owl:Class>
    


    <!-- http://tw.rpi.edu/web/Courses/Ontologies/2016/OE_8_TeaTeam/MaceFlavor -->

    <owl:Class rdf:about="http://tw.rpi.edu/web/Courses/Ontologies/2016/OE_8_TeaTeam/MaceFlavor">
        <rdfs:subClassOf rdf:resource="http://tw.rpi.edu/web/Courses/Ontologies/2016/OE_8_TeaTeam/ASTASpiceFlavor"/>
        <rdfs:subClassOf rdf:resource="http://tw.rpi.edu/web/Courses/Ontologies/2016/OE_8_TeaTeam/SpicyFlavor"/>
        <rdfs:comment>a flavor listed in the ASTA list that is reminiscent of mace, the dried covering or aril of the nutmeg seed, in one of several species in the genus Myristica</rdfs:comment>
        <rdfs:label xml:lang="en">mace flavor</rdfs:label>
    </owl:Class>
    


    <!-- http://tw.rpi.edu/web/Courses/Ontologies/2016/OE_8_TeaTeam/MajoramLeafFlavor -->

    <owl:Class rdf:about="http://tw.rpi.edu/web/Courses/Ontologies/2016/OE_8_TeaTeam/MajoramLeafFlavor">
        <rdfs:subClassOf rdf:resource="http://tw.rpi.edu/web/Courses/Ontologies/2016/OE_8_TeaTeam/ASTASpiceFlavor"/>
        <rdfs:subClassOf rdf:resource="http://tw.rpi.edu/web/Courses/Ontologies/2016/OE_8_TeaTeam/HerbalFlavor"/>
        <rdfs:comment>a flavor listed in the ASTA list that is reminiscent of majorum, the leaves of the herb Origanum majorana</rdfs:comment>
        <rdfs:label xml:lang="en">majoram leaf flavor</rdfs:label>
    </owl:Class>
    


    <!-- http://tw.rpi.edu/web/Courses/Ontologies/2016/OE_8_TeaTeam/MarineFlavor -->

    <owl:Class rdf:about="http://tw.rpi.edu/web/Courses/Ontologies/2016/OE_8_TeaTeam/MarineFlavor">
        <rdfs:subClassOf rdf:resource="http://tw.rpi.edu/web/Courses/Ontologies/2016/OE_8_TeaTeam/Flavor"/>
        <rdfs:comment xml:lang="en">a flavor that is salty, fishy, or evocative of the sea</rdfs:comment>
        <rdfs:label xml:lang="en">marine flavor</rdfs:label>
    </owl:Class>
    


    <!-- http://tw.rpi.edu/web/Courses/Ontologies/2016/OE_8_TeaTeam/MediumBrewingTemperature -->

    <owl:Class rdf:about="http://tw.rpi.edu/web/Courses/Ontologies/2016/OE_8_TeaTeam/MediumBrewingTemperature">
        <rdfs:subClassOf rdf:resource="http://tw.rpi.edu/web/Courses/Ontologies/2016/OE_8_TeaTeam/BrewingTemperature"/>
        <rdfs:comment>185~205°F or 85~96°C</rdfs:comment>
        <rdfs:label xml:lang="en">medium brewing temperature</rdfs:label>
    </owl:Class>
    


    <!-- http://tw.rpi.edu/web/Courses/Ontologies/2016/OE_8_TeaTeam/MintTea -->

    <owl:Class rdf:about="http://tw.rpi.edu/web/Courses/Ontologies/2016/OE_8_TeaTeam/MintTea">
        <rdfs:subClassOf rdf:resource="http://tw.rpi.edu/web/Courses/Ontologies/2016/OE_8_TeaTeam/DecaffeinatedSteepedDrink"/>
        <rdfs:subClassOf rdf:resource="http://tw.rpi.edu/web/Courses/Ontologies/2016/OE_8_TeaTeam/Tisane"/>
        <rdfs:subClassOf>
            <owl:Restriction>
                <owl:onProperty rdf:resource="http://tw.rpi.edu/web/Courses/Ontologies/2016/OE_8_TeaTeam/madeFromPart"/>
                <owl:someValuesFrom rdf:resource="http://tw.rpi.edu/web/Courses/Ontologies/2016/OE_8_TeaTeam/LeafPart"/>
            </owl:Restriction>
        </rdfs:subClassOf>
        <rdfs:comment>a tisane made from the leaves of plants in the Mentha family</rdfs:comment>
        <rdfs:label xml:lang="en">mint tea</rdfs:label>
    </owl:Class>
    


    <!-- http://tw.rpi.edu/web/Courses/Ontologies/2016/OE_8_TeaTeam/MustardSeedFlavor -->

    <owl:Class rdf:about="http://tw.rpi.edu/web/Courses/Ontologies/2016/OE_8_TeaTeam/MustardSeedFlavor">
        <rdfs:subClassOf rdf:resource="http://tw.rpi.edu/web/Courses/Ontologies/2016/OE_8_TeaTeam/ASTASpiceFlavor"/>
        <rdfs:subClassOf rdf:resource="http://tw.rpi.edu/web/Courses/Ontologies/2016/OE_8_TeaTeam/SpicyFlavor"/>
        <rdfs:comment>a flavor listed in the ASTA list that is reminiscent of mustard seed, the seed of either Brassica nigra, Brassica juncea, or Brassica alba/Sinapis alba</rdfs:comment>
        <rdfs:label xml:lang="en">mustard seed flavor</rdfs:label>
    </owl:Class>
    


    <!-- http://tw.rpi.edu/web/Courses/Ontologies/2016/OE_8_TeaTeam/NutmegFlavor -->

    <owl:Class rdf:about="http://tw.rpi.edu/web/Courses/Ontologies/2016/OE_8_TeaTeam/NutmegFlavor">
        <rdfs:subClassOf rdf:resource="http://tw.rpi.edu/web/Courses/Ontologies/2016/OE_8_TeaTeam/ASTASpiceFlavor"/>
        <rdfs:subClassOf rdf:resource="http://tw.rpi.edu/web/Courses/Ontologies/2016/OE_8_TeaTeam/SpicyFlavor"/>
        <rdfs:comment>a flavor listed in the ASTA list that is reminiscent of nutmeg, the seed of the nutmeg tree, from one of several species in the genus Myristica</rdfs:comment>
        <rdfs:label xml:lang="en">nutmeg flavor</rdfs:label>
    </owl:Class>
    


    <!-- http://tw.rpi.edu/web/Courses/Ontologies/2016/OE_8_TeaTeam/NuttyFlavor -->

    <owl:Class rdf:about="http://tw.rpi.edu/web/Courses/Ontologies/2016/OE_8_TeaTeam/NuttyFlavor">
        <rdfs:subClassOf rdf:resource="http://tw.rpi.edu/web/Courses/Ontologies/2016/OE_8_TeaTeam/Flavor"/>
        <rdfs:comment xml:lang="en">a flavor that is evocative of nuts</rdfs:comment>
        <rdfs:label xml:lang="en">nutty flavor</rdfs:label>
    </owl:Class>
    


    <!-- http://tw.rpi.edu/web/Courses/Ontologies/2016/OE_8_TeaTeam/OolongTea -->

    <owl:Class rdf:about="http://tw.rpi.edu/web/Courses/Ontologies/2016/OE_8_TeaTeam/OolongTea">
        <rdfs:subClassOf rdf:resource="http://tw.rpi.edu/web/Courses/Ontologies/2016/OE_8_TeaTeam/Tea"/>
        <rdfs:comment>Tea that has been withered, rolled, oxidized, and dried; partially but not completely oxidized</rdfs:comment>
        <rdfs:label xml:lang="en">oolong tea</rdfs:label>
    </owl:Class>
    


    <!-- http://tw.rpi.edu/web/Courses/Ontologies/2016/OE_8_TeaTeam/OreganoLeafFlavor -->

    <owl:Class rdf:about="http://tw.rpi.edu/web/Courses/Ontologies/2016/OE_8_TeaTeam/OreganoLeafFlavor">
        <rdfs:subClassOf rdf:resource="http://tw.rpi.edu/web/Courses/Ontologies/2016/OE_8_TeaTeam/ASTASpiceFlavor"/>
        <rdfs:subClassOf rdf:resource="http://tw.rpi.edu/web/Courses/Ontologies/2016/OE_8_TeaTeam/HerbalFlavor"/>
        <rdfs:comment>a flavor listed in the ASTA list that is reminiscent of oregano, the leaves of Origanum vulgare</rdfs:comment>
        <rdfs:label xml:lang="en">oregano flavor</rdfs:label>
    </owl:Class>
    


    <!-- http://tw.rpi.edu/web/Courses/Ontologies/2016/OE_8_TeaTeam/PaprikaFlavor -->

    <owl:Class rdf:about="http://tw.rpi.edu/web/Courses/Ontologies/2016/OE_8_TeaTeam/PaprikaFlavor">
        <rdfs:subClassOf rdf:resource="http://tw.rpi.edu/web/Courses/Ontologies/2016/OE_8_TeaTeam/ASTASpiceFlavor"/>
        <rdfs:subClassOf rdf:resource="http://tw.rpi.edu/web/Courses/Ontologies/2016/OE_8_TeaTeam/SpicyFlavor"/>
        <rdfs:comment>a flavor listed in the ASTA list that is reminiscent of paprika, the dried fruit of the plant Capsicum annuum</rdfs:comment>
        <rdfs:label xml:lang="en">paprika flavor</rdfs:label>
    </owl:Class>
    


    <!-- http://tw.rpi.edu/web/Courses/Ontologies/2016/OE_8_TeaTeam/ParsleyFlavor -->

    <owl:Class rdf:about="http://tw.rpi.edu/web/Courses/Ontologies/2016/OE_8_TeaTeam/ParsleyFlavor">
        <rdfs:subClassOf rdf:resource="http://tw.rpi.edu/web/Courses/Ontologies/2016/OE_8_TeaTeam/ASTASpiceFlavor"/>
        <rdfs:subClassOf rdf:resource="http://tw.rpi.edu/web/Courses/Ontologies/2016/OE_8_TeaTeam/HerbalFlavor"/>
        <rdfs:comment>a flavor listed in the ASTA list that is reminiscent of parsley, the leaves of the plant Petroselinum crispum</rdfs:comment>
        <rdfs:label xml:lang="en">parsley flavor</rdfs:label>
    </owl:Class>
    


    <!-- http://tw.rpi.edu/web/Courses/Ontologies/2016/OE_8_TeaTeam/PeppermintLeafFlavor -->

    <owl:Class rdf:about="http://tw.rpi.edu/web/Courses/Ontologies/2016/OE_8_TeaTeam/PeppermintLeafFlavor">
        <rdfs:subClassOf rdf:resource="http://tw.rpi.edu/web/Courses/Ontologies/2016/OE_8_TeaTeam/ASTASpiceFlavor"/>
        <rdfs:subClassOf rdf:resource="http://tw.rpi.edu/web/Courses/Ontologies/2016/OE_8_TeaTeam/HerbalFlavor"/>
        <rdfs:comment>a flavor listed in the ASTA list that is reminiscent of peppermint, the leaves of Mentha x piperita, a hybrid between Mentha aquatica and Mentha spicata</rdfs:comment>
        <rdfs:label xml:lang="en">pepperment leaf flavor</rdfs:label>
    </owl:Class>
    


    <!-- http://tw.rpi.edu/web/Courses/Ontologies/2016/OE_8_TeaTeam/PinkPeppercornFlavor -->

    <owl:Class rdf:about="http://tw.rpi.edu/web/Courses/Ontologies/2016/OE_8_TeaTeam/PinkPeppercornFlavor">
        <rdfs:subClassOf rdf:resource="http://tw.rpi.edu/web/Courses/Ontologies/2016/OE_8_TeaTeam/ASTASpiceFlavor"/>
        <rdfs:subClassOf rdf:resource="http://tw.rpi.edu/web/Courses/Ontologies/2016/OE_8_TeaTeam/SpicyFlavor"/>
        <rdfs:comment>a flavor listed in the ASTA list that is reminiscent of pink peppercorn, the dried berry of the shrub Schinus molle</rdfs:comment>
        <rdfs:label xml:lang="en">pink peppercorn flavor</rdfs:label>
    </owl:Class>
    


    <!-- http://tw.rpi.edu/web/Courses/Ontologies/2016/OE_8_TeaTeam/PlantPart -->

    <owl:Class rdf:about="http://tw.rpi.edu/web/Courses/Ontologies/2016/OE_8_TeaTeam/PlantPart">
        <rdfs:subClassOf rdf:resource="http://tw.rpi.edu/web/Courses/Ontologies/2016/OE_8_TeaTeam/DomainConcept"/>
        <rdfs:comment xml:lang="en">a part of a plant, defined culinarily, not botanically</rdfs:comment>
        <rdfs:label xml:lang="en">plant part</rdfs:label>
    </owl:Class>
    


    <!-- http://tw.rpi.edu/web/Courses/Ontologies/2016/OE_8_TeaTeam/PoppySeedFlavor -->

    <owl:Class rdf:about="http://tw.rpi.edu/web/Courses/Ontologies/2016/OE_8_TeaTeam/PoppySeedFlavor">
        <rdfs:subClassOf rdf:resource="http://tw.rpi.edu/web/Courses/Ontologies/2016/OE_8_TeaTeam/ASTASpiceFlavor"/>
        <rdfs:subClassOf rdf:resource="http://tw.rpi.edu/web/Courses/Ontologies/2016/OE_8_TeaTeam/SpicyFlavor"/>
        <rdfs:comment>a flavor listed in the ASTA list that is reminiscent of poppy seed, the seed of the flower Papaver somniferum</rdfs:comment>
        <rdfs:label xml:lang="en">poppy seed flavor</rdfs:label>
    </owl:Class>
    


    <!-- http://tw.rpi.edu/web/Courses/Ontologies/2016/OE_8_TeaTeam/Pu-ErhTea -->

    <owl:Class rdf:about="http://tw.rpi.edu/web/Courses/Ontologies/2016/OE_8_TeaTeam/Pu-ErhTea">
        <rdfs:subClassOf rdf:resource="http://tw.rpi.edu/web/Courses/Ontologies/2016/OE_8_TeaTeam/Tea"/>
        <rdfs:comment>Tea that is fermented, made from large tea leaves from older plants</rdfs:comment>
        <rdfs:label xml:lang="en">pu-erh tea</rdfs:label>
    </owl:Class>
    


    <!-- http://tw.rpi.edu/web/Courses/Ontologies/2016/OE_8_TeaTeam/RipePu-ErhTea -->

    <owl:Class rdf:about="http://tw.rpi.edu/web/Courses/Ontologies/2016/OE_8_TeaTeam/RipePu-ErhTea">
        <rdfs:subClassOf rdf:resource="http://tw.rpi.edu/web/Courses/Ontologies/2016/OE_8_TeaTeam/Pu-ErhTea"/>
        <rdfs:subClassOf>
            <owl:Restriction>
                <owl:onProperty rdf:resource="http://tw.rpi.edu/web/Courses/Ontologies/2016/OE_8_TeaTeam/hasBrewingTemperature"/>
                <owl:someValuesFrom rdf:resource="http://tw.rpi.edu/web/Courses/Ontologies/2016/OE_8_TeaTeam/HighBrewingTemperature"/>
            </owl:Restriction>
        </rdfs:subClassOf>
        <rdfs:comment>A pu-erh tea that is piled and left to ferment after processing</rdfs:comment>
        <rdfs:label xml:lang="en">ripe pu-erh tea</rdfs:label>
    </owl:Class>
    


    <!-- http://tw.rpi.edu/web/Courses/Ontologies/2016/OE_8_TeaTeam/RooibosTea -->

    <owl:Class rdf:about="http://tw.rpi.edu/web/Courses/Ontologies/2016/OE_8_TeaTeam/RooibosTea">
        <rdfs:subClassOf rdf:resource="http://tw.rpi.edu/web/Courses/Ontologies/2016/OE_8_TeaTeam/DecaffeinatedSteepedDrink"/>
        <rdfs:subClassOf rdf:resource="http://tw.rpi.edu/web/Courses/Ontologies/2016/OE_8_TeaTeam/Tisane"/>
        <rdfs:comment>A steeped drink made from the leaves of Aspalanthus linearis, grown in South Africa. Contains no caffeine.</rdfs:comment>
        <rdfs:label xml:lang="en">rooibos tea</rdfs:label>
    </owl:Class>
    


    <!-- http://tw.rpi.edu/web/Courses/Ontologies/2016/OE_8_TeaTeam/RootPart -->

    <owl:Class rdf:about="http://tw.rpi.edu/web/Courses/Ontologies/2016/OE_8_TeaTeam/RootPart">
        <rdfs:subClassOf rdf:resource="http://tw.rpi.edu/web/Courses/Ontologies/2016/OE_8_TeaTeam/PlantPart"/>
        <rdfs:subClassOf>
            <owl:Restriction>
                <owl:onProperty rdf:resource="http://tw.rpi.edu/web/Courses/Ontologies/2016/OE_8_TeaTeam/brewsAt"/>
                <owl:someValuesFrom rdf:resource="http://tw.rpi.edu/web/Courses/Ontologies/2016/OE_8_TeaTeam/HighBrewingTemperature"/>
            </owl:Restriction>
        </rdfs:subClassOf>
        <rdfs:comment>an underground part of a plant, used for gathering nutrients, storing nutrients, or for supporting the plant</rdfs:comment>
        <rdfs:label xml:lang="en">root part</rdfs:label>
    </owl:Class>
    


    <!-- http://tw.rpi.edu/web/Courses/Ontologies/2016/OE_8_TeaTeam/RosemaryFlavor -->

    <owl:Class rdf:about="http://tw.rpi.edu/web/Courses/Ontologies/2016/OE_8_TeaTeam/RosemaryFlavor">
        <rdfs:subClassOf rdf:resource="http://tw.rpi.edu/web/Courses/Ontologies/2016/OE_8_TeaTeam/ASTASpiceFlavor"/>
        <rdfs:subClassOf rdf:resource="http://tw.rpi.edu/web/Courses/Ontologies/2016/OE_8_TeaTeam/HerbalFlavor"/>
        <rdfs:comment>a flavor listed in the ASTA list that is reminiscent of rosemary, the leaves of the herb Rosmarinus officinalis</rdfs:comment>
        <rdfs:label xml:lang="en">rosemary flavor</rdfs:label>
    </owl:Class>
    


    <!-- http://tw.rpi.edu/web/Courses/Ontologies/2016/OE_8_TeaTeam/SageFlavor -->

    <owl:Class rdf:about="http://tw.rpi.edu/web/Courses/Ontologies/2016/OE_8_TeaTeam/SageFlavor">
        <rdfs:subClassOf rdf:resource="http://tw.rpi.edu/web/Courses/Ontologies/2016/OE_8_TeaTeam/ASTASpiceFlavor"/>
        <rdfs:subClassOf rdf:resource="http://tw.rpi.edu/web/Courses/Ontologies/2016/OE_8_TeaTeam/HerbalFlavor"/>
        <rdfs:comment>a flavor listed in the ASTA list that is reminiscent of sage, the leaves of the plant Salvia officinalis</rdfs:comment>
        <rdfs:label xml:lang="en">sage flavor</rdfs:label>
    </owl:Class>
    


    <!-- http://tw.rpi.edu/web/Courses/Ontologies/2016/OE_8_TeaTeam/SavoryLeafFlavor -->

    <owl:Class rdf:about="http://tw.rpi.edu/web/Courses/Ontologies/2016/OE_8_TeaTeam/SavoryLeafFlavor">
        <rdfs:subClassOf rdf:resource="http://tw.rpi.edu/web/Courses/Ontologies/2016/OE_8_TeaTeam/ASTASpiceFlavor"/>
        <rdfs:subClassOf rdf:resource="http://tw.rpi.edu/web/Courses/Ontologies/2016/OE_8_TeaTeam/HerbalFlavor"/>
        <rdfs:comment>a flavor listed in the ASTA list that is reminiscent of savory, the leaves of the plant Satureja hortensis or Satureja montana</rdfs:comment>
        <rdfs:label xml:lang="en">savory leaf flavor</rdfs:label>
    </owl:Class>
    


    <!-- http://tw.rpi.edu/web/Courses/Ontologies/2016/OE_8_TeaTeam/SeedPart -->

    <owl:Class rdf:about="http://tw.rpi.edu/web/Courses/Ontologies/2016/OE_8_TeaTeam/SeedPart">
        <rdfs:subClassOf rdf:resource="http://tw.rpi.edu/web/Courses/Ontologies/2016/OE_8_TeaTeam/PlantPart"/>
        <rdfs:subClassOf>
            <owl:Restriction>
                <owl:onProperty rdf:resource="http://tw.rpi.edu/web/Courses/Ontologies/2016/OE_8_TeaTeam/brewsAt"/>
                <owl:someValuesFrom rdf:resource="http://tw.rpi.edu/web/Courses/Ontologies/2016/OE_8_TeaTeam/HighBrewingTemperature"/>
            </owl:Restriction>
        </rdfs:subClassOf>
        <rdfs:comment>the developed, fertilized part of a flowering plant</rdfs:comment>
        <rdfs:label xml:lang="en">seed part</rdfs:label>
    </owl:Class>
    


    <!-- http://tw.rpi.edu/web/Courses/Ontologies/2016/OE_8_TeaTeam/SenchaGreenTea -->

    <owl:Class rdf:about="http://tw.rpi.edu/web/Courses/Ontologies/2016/OE_8_TeaTeam/SenchaGreenTea">
        <rdfs:subClassOf rdf:resource="http://tw.rpi.edu/web/Courses/Ontologies/2016/OE_8_TeaTeam/GreenTea"/>
        <rdfs:comment>A green tea from Japan produced from unshaded steamed leaves picked during spring</rdfs:comment>
        <rdfs:label xml:lang="en">sencha green tea</rdfs:label>
    </owl:Class>
    


    <!-- http://tw.rpi.edu/web/Courses/Ontologies/2016/OE_8_TeaTeam/SesameSeedFlavor -->

    <owl:Class rdf:about="http://tw.rpi.edu/web/Courses/Ontologies/2016/OE_8_TeaTeam/SesameSeedFlavor">
        <rdfs:subClassOf rdf:resource="http://tw.rpi.edu/web/Courses/Ontologies/2016/OE_8_TeaTeam/ASTASpiceFlavor"/>
        <rdfs:subClassOf rdf:resource="http://tw.rpi.edu/web/Courses/Ontologies/2016/OE_8_TeaTeam/SpicyFlavor"/>
        <rdfs:comment>a flavor listed in the ASTA list that is reminiscent of sesame seed, the seed of the plant Sesamum indicum</rdfs:comment>
        <rdfs:label xml:lang="en">sesame seed flavor</rdfs:label>
    </owl:Class>
    


    <!-- http://tw.rpi.edu/web/Courses/Ontologies/2016/OE_8_TeaTeam/SpearmintFlavor -->

    <owl:Class rdf:about="http://tw.rpi.edu/web/Courses/Ontologies/2016/OE_8_TeaTeam/SpearmintFlavor">
        <rdfs:subClassOf rdf:resource="http://tw.rpi.edu/web/Courses/Ontologies/2016/OE_8_TeaTeam/ASTASpiceFlavor"/>
        <rdfs:subClassOf rdf:resource="http://tw.rpi.edu/web/Courses/Ontologies/2016/OE_8_TeaTeam/HerbalFlavor"/>
        <rdfs:comment>a flavor listed in the ASTA list that is reminiscent of spearmint, the leaves of the plant Mentha spicata</rdfs:comment>
        <rdfs:label xml:lang="en">spearmint flavor</rdfs:label>
    </owl:Class>
    


    <!-- http://tw.rpi.edu/web/Courses/Ontologies/2016/OE_8_TeaTeam/SpicyFlavor -->

    <owl:Class rdf:about="http://tw.rpi.edu/web/Courses/Ontologies/2016/OE_8_TeaTeam/SpicyFlavor">
        <rdfs:subClassOf rdf:resource="http://tw.rpi.edu/web/Courses/Ontologies/2016/OE_8_TeaTeam/Flavor"/>
        <rdfs:comment xml:lang="en">a flavor that is evocative of culinary/medicinal spices - aromatic substances obtained from roots, flowers, fruits, seeds or bark; not necessarily capsaicin</rdfs:comment>
        <rdfs:label xml:lang="en">spicy flavor</rdfs:label>
    </owl:Class>
    


    <!-- http://tw.rpi.edu/web/Courses/Ontologies/2016/OE_8_TeaTeam/StarAniseFlavor -->

    <owl:Class rdf:about="http://tw.rpi.edu/web/Courses/Ontologies/2016/OE_8_TeaTeam/StarAniseFlavor">
        <rdfs:subClassOf rdf:resource="http://tw.rpi.edu/web/Courses/Ontologies/2016/OE_8_TeaTeam/ASTASpiceFlavor"/>
        <rdfs:subClassOf rdf:resource="http://tw.rpi.edu/web/Courses/Ontologies/2016/OE_8_TeaTeam/SpicyFlavor"/>
        <rdfs:comment>a flavor listed in the ASTA list that is reminiscent of star anise, the fruit of the tree Illicium verum</rdfs:comment>
        <rdfs:label xml:lang="en">star anise flavor</rdfs:label>
    </owl:Class>
    


    <!-- http://tw.rpi.edu/web/Courses/Ontologies/2016/OE_8_TeaTeam/SteepedDrink -->

    <owl:Class rdf:about="http://tw.rpi.edu/web/Courses/Ontologies/2016/OE_8_TeaTeam/SteepedDrink">
        <owl:equivalentClass>
            <owl:Restriction>
                <owl:onProperty rdf:resource="http://tw.rpi.edu/web/Courses/Ontologies/2016/OE_8_TeaTeam/hasBrewingTemperature"/>
                <owl:minQualifiedCardinality rdf:datatype="http://www.w3.org/2001/XMLSchema#nonNegativeInteger">1</owl:minQualifiedCardinality>
                <owl:onClass rdf:resource="http://tw.rpi.edu/web/Courses/Ontologies/2016/OE_8_TeaTeam/BrewingTemperature"/>
            </owl:Restriction>
        </owl:equivalentClass>
        <owl:equivalentClass>
            <owl:Restriction>
                <owl:onProperty rdf:resource="http://tw.rpi.edu/web/Courses/Ontologies/2016/OE_8_TeaTeam/hasFlavor"/>
                <owl:minQualifiedCardinality rdf:datatype="http://www.w3.org/2001/XMLSchema#nonNegativeInteger">1</owl:minQualifiedCardinality>
                <owl:onClass rdf:resource="http://tw.rpi.edu/web/Courses/Ontologies/2016/OE_8_TeaTeam/Flavor"/>
            </owl:Restriction>
        </owl:equivalentClass>
        <rdfs:subClassOf rdf:resource="http://tw.rpi.edu/web/Courses/Ontologies/2016/OE_8_TeaTeam/DomainConcept"/>
        <rdfs:comment xml:lang="en">A beverage that has been prepared by allowing ingredients to soak in water at a temperature under the boiling point.</rdfs:comment>
        <rdfs:label xml:lang="en">steeped drink</rdfs:label>
    </owl:Class>
    


    <!-- http://tw.rpi.edu/web/Courses/Ontologies/2016/OE_8_TeaTeam/SweetFlavor -->

    <owl:Class rdf:about="http://tw.rpi.edu/web/Courses/Ontologies/2016/OE_8_TeaTeam/SweetFlavor">
        <rdfs:subClassOf rdf:resource="http://tw.rpi.edu/web/Courses/Ontologies/2016/OE_8_TeaTeam/Flavor"/>
        <rdfs:comment xml:lang="en">a flavor that is sugary or syrupy</rdfs:comment>
        <rdfs:label xml:lang="en">sweet flavor</rdfs:label>
    </owl:Class>
    


    <!-- http://tw.rpi.edu/web/Courses/Ontologies/2016/OE_8_TeaTeam/TarragonFlavor -->

    <owl:Class rdf:about="http://tw.rpi.edu/web/Courses/Ontologies/2016/OE_8_TeaTeam/TarragonFlavor">
        <rdfs:subClassOf rdf:resource="http://tw.rpi.edu/web/Courses/Ontologies/2016/OE_8_TeaTeam/ASTASpiceFlavor"/>
        <rdfs:subClassOf rdf:resource="http://tw.rpi.edu/web/Courses/Ontologies/2016/OE_8_TeaTeam/HerbalFlavor"/>
        <rdfs:comment>a flavor listed in the ASTA list that is reminiscent of tarragon, the leaves of the herb Artemisia dracunculus</rdfs:comment>
        <rdfs:label xml:lang="en">tarragon flavor</rdfs:label>
    </owl:Class>
    


    <!-- http://tw.rpi.edu/web/Courses/Ontologies/2016/OE_8_TeaTeam/Tea -->

    <owl:Class rdf:about="http://tw.rpi.edu/web/Courses/Ontologies/2016/OE_8_TeaTeam/Tea">
        <rdfs:subClassOf rdf:resource="http://tw.rpi.edu/web/Courses/Ontologies/2016/OE_8_TeaTeam/CaffeinatedSteepedDrink"/>
        <rdfs:comment>A steeped drink made from the leaves of the Camellia sinensis plant</rdfs:comment>
        <rdfs:label xml:lang="en">tea</rdfs:label>
    </owl:Class>
    


    <!-- http://tw.rpi.edu/web/Courses/Ontologies/2016/OE_8_TeaTeam/ThymeFlavor -->

    <owl:Class rdf:about="http://tw.rpi.edu/web/Courses/Ontologies/2016/OE_8_TeaTeam/ThymeFlavor">
        <rdfs:subClassOf rdf:resource="http://tw.rpi.edu/web/Courses/Ontologies/2016/OE_8_TeaTeam/ASTASpiceFlavor"/>
        <rdfs:subClassOf rdf:resource="http://tw.rpi.edu/web/Courses/Ontologies/2016/OE_8_TeaTeam/HerbalFlavor"/>
        <rdfs:comment>a flavor listed in the ASTA list that is reminiscent of thyme, the leaves of the plant Thymus vulgaris</rdfs:comment>
        <rdfs:label xml:lang="en">thyme flavor</rdfs:label>
    </owl:Class>
    


    <!-- http://tw.rpi.edu/web/Courses/Ontologies/2016/OE_8_TeaTeam/Tisane -->

    <owl:Class rdf:about="http://tw.rpi.edu/web/Courses/Ontologies/2016/OE_8_TeaTeam/Tisane">
        <rdfs:subClassOf rdf:resource="http://tw.rpi.edu/web/Courses/Ontologies/2016/OE_8_TeaTeam/SteepedDrink"/>
        <rdfs:comment>A steeped drink made from plants other than Camellia sinensis</rdfs:comment>
        <rdfs:label xml:lang="en">tisane</rdfs:label>
    </owl:Class>
    


    <!-- http://tw.rpi.edu/web/Courses/Ontologies/2016/OE_8_TeaTeam/ValuePartition -->

    <owl:Class rdf:about="http://tw.rpi.edu/web/Courses/Ontologies/2016/OE_8_TeaTeam/ValuePartition">
        <rdfs:label xml:lang="en">value partition</rdfs:label>
    </owl:Class>
    


    <!-- http://tw.rpi.edu/web/Courses/Ontologies/2016/OE_8_TeaTeam/VanillaFlavor -->

    <owl:Class rdf:about="http://tw.rpi.edu/web/Courses/Ontologies/2016/OE_8_TeaTeam/VanillaFlavor">
        <rdfs:subClassOf rdf:resource="http://tw.rpi.edu/web/Courses/Ontologies/2016/OE_8_TeaTeam/ASTASpiceFlavor"/>
        <rdfs:subClassOf rdf:resource="http://tw.rpi.edu/web/Courses/Ontologies/2016/OE_8_TeaTeam/SweetFlavor"/>
        <rdfs:comment>a flavor listed in the ASTA list that is reminiscent of vanilla, the seed pods of flowering vines in the genus Vanilla, typically Vanilla planifolia</rdfs:comment>
        <rdfs:label xml:lang="en">vanilla flavor</rdfs:label>
    </owl:Class>
    


    <!-- http://tw.rpi.edu/web/Courses/Ontologies/2016/OE_8_TeaTeam/VegetalFlavor -->

    <owl:Class rdf:about="http://tw.rpi.edu/web/Courses/Ontologies/2016/OE_8_TeaTeam/VegetalFlavor">
        <rdfs:subClassOf rdf:resource="http://tw.rpi.edu/web/Courses/Ontologies/2016/OE_8_TeaTeam/Flavor"/>
        <rdfs:comment xml:lang="en">a flavor that is leafy, grassy, or evocative of a vegetable</rdfs:comment>
        <rdfs:label xml:lang="en">vegetal flavor</rdfs:label>
    </owl:Class>
    


    <!-- http://tw.rpi.edu/web/Courses/Ontologies/2016/OE_8_TeaTeam/WhitePepperFlavor -->

    <owl:Class rdf:about="http://tw.rpi.edu/web/Courses/Ontologies/2016/OE_8_TeaTeam/WhitePepperFlavor">
        <rdfs:subClassOf rdf:resource="http://tw.rpi.edu/web/Courses/Ontologies/2016/OE_8_TeaTeam/ASTASpiceFlavor"/>
        <rdfs:subClassOf rdf:resource="http://tw.rpi.edu/web/Courses/Ontologies/2016/OE_8_TeaTeam/SpicyFlavor"/>
        <rdfs:comment>a flavor listed in the ASTA list that is reminiscent of white pepper, the seeds of the plant Piper nigrum that has had the skin of the fruit removed</rdfs:comment>
        <rdfs:label xml:lang="en">white pepper flavor</rdfs:label>
    </owl:Class>
    


    <!-- http://tw.rpi.edu/web/Courses/Ontologies/2016/OE_8_TeaTeam/WhiteTea -->

    <owl:Class rdf:about="http://tw.rpi.edu/web/Courses/Ontologies/2016/OE_8_TeaTeam/WhiteTea">
        <rdfs:subClassOf rdf:resource="http://tw.rpi.edu/web/Courses/Ontologies/2016/OE_8_TeaTeam/Tea"/>
        <rdfs:comment>Tea that has been dried, but not withered, rolled, or oxidized</rdfs:comment>
        <rdfs:label xml:lang="en">white tea</rdfs:label>
    </owl:Class>
    


    <!-- http://tw.rpi.edu/web/Courses/Ontologies/2016/OE_8_TeaTeam/WoodyFlavor -->

    <owl:Class rdf:about="http://tw.rpi.edu/web/Courses/Ontologies/2016/OE_8_TeaTeam/WoodyFlavor">
        <rdfs:subClassOf rdf:resource="http://tw.rpi.edu/web/Courses/Ontologies/2016/OE_8_TeaTeam/Flavor"/>
        <rdfs:comment xml:lang="en">a flavor that is evocative of wood or trees</rdfs:comment>
        <rdfs:label xml:lang="en">woody flavor</rdfs:label>
    </owl:Class>
    


    <!-- http://tw.rpi.edu/web/Courses/Ontologies/2016/OE_8_TeaTeam/YerbaMate -->

    <owl:Class rdf:about="http://tw.rpi.edu/web/Courses/Ontologies/2016/OE_8_TeaTeam/YerbaMate">
        <rdfs:subClassOf rdf:resource="http://tw.rpi.edu/web/Courses/Ontologies/2016/OE_8_TeaTeam/CaffeinatedSteepedDrink"/>
        <rdfs:subClassOf rdf:resource="http://tw.rpi.edu/web/Courses/Ontologies/2016/OE_8_TeaTeam/Tisane"/>
        <rdfs:comment>A steeped drink made from the leaves of Ilex paraguariensis, grown in South America. Contains caffeine.</rdfs:comment>
        <rdfs:label xml:lang="en">yerba mate</rdfs:label>
    </owl:Class>
    


    <!-- http://tw.rpi.edu/web/Courses/Ontologies/2016/OE_8_TeaTeam/YoungRawPu-ErhTea -->

    <owl:Class rdf:about="http://tw.rpi.edu/web/Courses/Ontologies/2016/OE_8_TeaTeam/YoungRawPu-ErhTea">
        <rdfs:subClassOf rdf:resource="http://tw.rpi.edu/web/Courses/Ontologies/2016/OE_8_TeaTeam/Pu-ErhTea"/>
        <rdfs:subClassOf>
            <owl:Restriction>
                <owl:onProperty rdf:resource="http://tw.rpi.edu/web/Courses/Ontologies/2016/OE_8_TeaTeam/hasBrewingTemperature"/>
                <owl:someValuesFrom rdf:resource="http://tw.rpi.edu/web/Courses/Ontologies/2016/OE_8_TeaTeam/MediumBrewingTemperature"/>
            </owl:Restriction>
        </rdfs:subClassOf>
        <rdfs:comment>A pu-erh tea that is less than three years old</rdfs:comment>
        <rdfs:label xml:lang="en">young raw pu-erh tea</rdfs:label>
    </owl:Class>
    


    <!-- http://www.nanopub.org/nschema#Assertion -->

    <owl:Class rdf:about="http://www.nanopub.org/nschema#Assertion">
        <rdfs:subClassOf rdf:resource="http://www.w3.org/2004/03/trix/rdfg-1/Graph"/>
        <rdfs:label xml:lang="en">Assertion</rdfs:label>
    </owl:Class>
    


    <!-- http://www.nanopub.org/nschema#Nanopublication -->

    <owl:Class rdf:about="http://www.nanopub.org/nschema#Nanopublication">
        <rdfs:label xml:lang="en">Nanopublication</rdfs:label>
    </owl:Class>
    


    <!-- http://www.w3.org/2004/03/trix/rdfg-1/Graph -->

    <owl:Class rdf:about="http://www.w3.org/2004/03/trix/rdfg-1/Graph"/>
</rdf:RDF>



<!-- Generated by the OWL API (version 4.2.1.20160306-0033) https://github.com/owlcs/owlapi -->

