<?xml version="1.0"?>


<!DOCTYPE rdf:RDF [
    <!ENTITY dct "http://purl.org/dc/terms/" >
    <!ENTITY owl "http://www.w3.org/2002/07/owl#" >
    <!ENTITY np "http://www.nanopub.org/nschema#" >
    <!ENTITY xsd "http://www.w3.org/2001/XMLSchema#" >
    <!ENTITY skos "http://www.w3.org/2004/02/skos/core#" >
    <!ENTITY rdfs "http://www.w3.org/2000/01/rdf-schema#" >
    <!ENTITY rdfg-1 "http://www.w3.org/2004/03/trix/rdfg-1/" >
    <!ENTITY rdf "http://www.w3.org/1999/02/22-rdf-syntax-ns#" >
    <!ENTITY tea "http://tw.rpi.edu/web/Courses/Ontologies/2016/OE_9_TeaTeam/" >
]>


<rdf:RDF xmlns="http://tw.rpi.edu/web/Courses/Ontologies/2016/OE_9_TeaTeam/"
     xml:base="http://tw.rpi.edu/web/Courses/Ontologies/2016/OE_9_TeaTeam/"
     xmlns:rdfg-1="http://www.w3.org/2004/03/trix/rdfg-1/"
     xmlns:rdfs="http://www.w3.org/2000/01/rdf-schema#"
     xmlns:np="http://www.nanopub.org/nschema#"
     xmlns:dct="http://purl.org/dc/terms/"
     xmlns:owl="http://www.w3.org/2002/07/owl#"
     xmlns:xsd="http://www.w3.org/2001/XMLSchema#"
     xmlns:rdf="http://www.w3.org/1999/02/22-rdf-syntax-ns#"
     xmlns:tea="http://tw.rpi.edu/web/Courses/Ontologies/2016/OE_9_TeaTeam/"
     xmlns:skos="http://www.w3.org/2004/02/skos/core#">
    <owl:Ontology rdf:about="http://tw.rpi.edu/web/Courses/Ontologies/2016/OE_9_TeaTeam/">
        <rdfs:label>Tea Ontology</rdfs:label>
        <dct:creator xml:lang="en">Cara Reedy</dct:creator>
        <dct:creator xml:lang="en">Katie Chastain</dct:creator>
        <owl:imports rdf:resource="http://www.nanopub.org/nschema#"/>
        <owl:imports rdf:resource="http://www.w3.org/2004/02/skos/core"/>
    </owl:Ontology>
    


    <!-- 
    ///////////////////////////////////////////////////////////////////////////////////////
    //
    // Annotation properties
    //
    ///////////////////////////////////////////////////////////////////////////////////////
     -->

    


    <!-- http://purl.org/dc/terms/abstract -->

    <owl:AnnotationProperty rdf:about="&dct;abstract"/>
    


    <!-- http://purl.org/dc/terms/contributor -->

    <owl:AnnotationProperty rdf:about="&dct;contributor"/>
    


    <!-- http://purl.org/dc/terms/creator -->

    <owl:AnnotationProperty rdf:about="&dct;creator"/>
    


    <!-- http://purl.org/dc/terms/description -->

    <owl:AnnotationProperty rdf:about="&dct;description"/>
    


    <!-- http://purl.org/dc/terms/format -->

    <owl:AnnotationProperty rdf:about="&dct;format"/>
    


    <!-- http://purl.org/dc/terms/hasVersion -->

    <owl:AnnotationProperty rdf:about="&dct;hasVersion"/>
    


    <!-- http://purl.org/dc/terms/identifier -->

    <owl:AnnotationProperty rdf:about="&dct;identifier"/>
    


    <!-- http://purl.org/dc/terms/issued -->

    <owl:AnnotationProperty rdf:about="&dct;issued"/>
    


    <!-- http://purl.org/dc/terms/license -->

    <owl:AnnotationProperty rdf:about="&dct;license"/>
    


    <!-- http://purl.org/dc/terms/references -->

    <owl:AnnotationProperty rdf:about="&dct;references"/>
    


    <!-- http://purl.org/dc/terms/rights -->

    <owl:AnnotationProperty rdf:about="&dct;rights"/>
    


    <!-- http://purl.org/dc/terms/source -->

    <owl:AnnotationProperty rdf:about="&dct;source"/>
    


    <!-- http://purl.org/dc/terms/subject -->

    <owl:AnnotationProperty rdf:about="&dct;subject"/>
    


    <!-- http://purl.org/dc/terms/title -->

    <owl:AnnotationProperty rdf:about="&dct;title"/>
    


    <!-- http://purl.org/dc/terms/type -->

    <owl:AnnotationProperty rdf:about="&dct;type"/>
    


    <!-- http://www.w3.org/2004/02/skos/core#altLabel -->

    <owl:AnnotationProperty rdf:about="&skos;altLabel"/>
    


    <!-- http://www.w3.org/2004/02/skos/core#changeNote -->

    <owl:AnnotationProperty rdf:about="&skos;changeNote"/>
    


    <!-- http://www.w3.org/2004/02/skos/core#definition -->

    <owl:AnnotationProperty rdf:about="&skos;definition"/>
    


    <!-- http://www.w3.org/2004/02/skos/core#editorialNote -->

    <owl:AnnotationProperty rdf:about="&skos;editorialNote"/>
    


    <!-- http://www.w3.org/2004/02/skos/core#example -->

    <owl:AnnotationProperty rdf:about="&skos;example"/>
    


    <!-- http://www.w3.org/2004/02/skos/core#historyNote -->

    <owl:AnnotationProperty rdf:about="&skos;historyNote"/>
    


    <!-- http://www.w3.org/2004/02/skos/core#note -->

    <owl:AnnotationProperty rdf:about="&skos;note"/>
    


    <!-- http://www.w3.org/2004/02/skos/core#prefLabel -->

    <owl:AnnotationProperty rdf:about="&skos;prefLabel"/>
    


    <!-- http://www.w3.org/2004/02/skos/core#scopeNote -->

    <owl:AnnotationProperty rdf:about="&skos;scopeNote"/>
    


    <!-- 
    ///////////////////////////////////////////////////////////////////////////////////////
    //
    // Object Properties
    //
    ///////////////////////////////////////////////////////////////////////////////////////
     -->

    


    <!-- http://tw.rpi.edu/web/Courses/Ontologies/2016/OE_9_TeaTeam/brews -->

    <owl:ObjectProperty rdf:about="&tea;brews">
        <skos:definition>the steepedDrinks a particular brewing temperature range can steep</skos:definition>
        <rdfs:domain rdf:resource="&tea;BrewingTemperature"/>
        <owl:inverseOf rdf:resource="&tea;hasBrewingTemperature"/>
    </owl:ObjectProperty>
    


    <!-- http://tw.rpi.edu/web/Courses/Ontologies/2016/OE_9_TeaTeam/brewsAt -->

    <owl:ObjectProperty rdf:about="&tea;brewsAt">
        <skos:definition xml:lang="en">Relates a Plant Part to its appropriate Brewing Temperature(s)</skos:definition>
    </owl:ObjectProperty>
    


    <!-- http://tw.rpi.edu/web/Courses/Ontologies/2016/OE_9_TeaTeam/contains -->

    <owl:ObjectProperty rdf:about="&tea;contains">
        <skos:definition>used for blend to indicate which steepedDrinks are part of that blend</skos:definition>
    </owl:ObjectProperty>
    


    <!-- http://tw.rpi.edu/web/Courses/Ontologies/2016/OE_9_TeaTeam/flavorOf -->

    <owl:ObjectProperty rdf:about="&tea;flavorOf">
        <skos:definition>the steepedDrinks a particular flavor flavors</skos:definition>
        <owl:inverseOf rdf:resource="&tea;hasFlavor"/>
    </owl:ObjectProperty>
    


    <!-- http://tw.rpi.edu/web/Courses/Ontologies/2016/OE_9_TeaTeam/fromSource -->

    <owl:ObjectProperty rdf:about="&tea;fromSource"/>
    


    <!-- http://tw.rpi.edu/web/Courses/Ontologies/2016/OE_9_TeaTeam/hasBrewingTemperature -->

    <owl:ObjectProperty rdf:about="&tea;hasBrewingTemperature">
        <skos:definition>the brewing temperature range used for a particular steepedDrink</skos:definition>
        <rdfs:range rdf:resource="&tea;BrewingTemperature"/>
        <owl:propertyChainAxiom rdf:parseType="Collection">
            <rdf:Description rdf:about="&tea;madeFromPart"/>
            <rdf:Description rdf:about="&tea;brewsAt"/>
        </owl:propertyChainAxiom>
    </owl:ObjectProperty>
    


    <!-- http://tw.rpi.edu/web/Courses/Ontologies/2016/OE_9_TeaTeam/hasCaffeine -->

    <owl:ObjectProperty rdf:about="&tea;hasCaffeine">
        <skos:definition>has caffeination value of caffeine or no caffeine</skos:definition>
        <rdfs:range rdf:resource="&tea;Caffeination"/>
    </owl:ObjectProperty>
    


    <!-- http://tw.rpi.edu/web/Courses/Ontologies/2016/OE_9_TeaTeam/hasFlavor -->

    <owl:ObjectProperty rdf:about="&tea;hasFlavor">
        <skos:definition>the flavor of a particular steepedDrink</skos:definition>
    </owl:ObjectProperty>
    


    <!-- http://tw.rpi.edu/web/Courses/Ontologies/2016/OE_9_TeaTeam/madeFromPart -->

    <owl:ObjectProperty rdf:about="&tea;madeFromPart">
        <skos:definition>defines what kind of plant part a tisane is made from</skos:definition>
        <rdfs:range rdf:resource="&tea;PlantPart"/>
    </owl:ObjectProperty>
    


    <!-- http://tw.rpi.edu/web/Courses/Ontologies/2016/OE_9_TeaTeam/withStrength -->

    <owl:ObjectProperty rdf:about="&tea;withStrength">
        <rdfs:domain rdf:resource="&tea;FlavorCompatibility"/>
    </owl:ObjectProperty>
    


    <!-- 
    ///////////////////////////////////////////////////////////////////////////////////////
    //
    // Classes
    //
    ///////////////////////////////////////////////////////////////////////////////////////
     -->

    


    <!-- http://tw.rpi.edu/web/Courses/Ontologies/2016/OE_9_TeaTeam/ASTASpiceFlavor -->

    <owl:Class rdf:about="&tea;ASTASpiceFlavor">
        <rdfs:label xml:lang="en">ASTA spice flavor</rdfs:label>
        <rdfs:subClassOf rdf:resource="&tea;Flavor"/>
        <dct:source>ASTA spice list (http://www.astaspice.org/download/9423/)</dct:source>
        <skos:definition>a flavor which comes from a spice defined by the ASTA spice list</skos:definition>
    </owl:Class>
    


    <!-- http://tw.rpi.edu/web/Courses/Ontologies/2016/OE_9_TeaTeam/AgedRipePu-ErhTea -->

    <owl:Class rdf:about="&tea;AgedRipePu-ErhTea">
        <rdfs:label xml:lang="en">aged raw pu-erh tea</rdfs:label>
        <rdfs:subClassOf rdf:resource="&tea;Pu-ErhTea"/>
        <rdfs:subClassOf>
            <owl:Restriction>
                <owl:onProperty rdf:resource="&tea;hasBrewingTemperature"/>
                <owl:someValuesFrom rdf:resource="&tea;HighBrewingTemperature"/>
            </owl:Restriction>
        </rdfs:subClassOf>
        <dct:source>http://www.seriouseats.com/2015/08/what-is-puerh-tea-where-to-buy.html</dct:source>
        <skos:definition>A pu-erh tea that is at least three years old</skos:definition>
    </owl:Class>
    


    <!-- http://tw.rpi.edu/web/Courses/Ontologies/2016/OE_9_TeaTeam/AllspiceFlavor -->

    <owl:Class rdf:about="&tea;AllspiceFlavor">
        <rdfs:label xml:lang="en">allspice flavor</rdfs:label>
        <rdfs:subClassOf rdf:resource="&tea;ASTASpiceFlavor"/>
        <rdfs:subClassOf rdf:resource="&tea;SpicyFlavor"/>
        <dct:source>ASTA spice list (http://www.astaspice.org/download/9423/)</dct:source>
        <skos:definition>a flavor listed in the ASTA list that is reminiscent of allspice, the dried berries of Pimenta dioica</skos:definition>
    </owl:Class>
    


    <!-- http://tw.rpi.edu/web/Courses/Ontologies/2016/OE_9_TeaTeam/AnimalFlavor -->

    <owl:Class rdf:about="&tea;AnimalFlavor">
        <rdfs:label xml:lang="en">animal flavor</rdfs:label>
        <rdfs:subClassOf rdf:resource="&tea;Flavor"/>
        <dct:source>Adapted from Tea Cupping Standards (http://www.worldoftea.org/tea-cupping-standards/), Stone Leaf Tea&apos;s Tea Guru (http://www.stoneleaftea.com/tea-guru/), and The Australian Tea Maters&apos; Tea Flavour Wheel (https://australianteamasters.wordpress.com/2014/04/30/the-tea-flavour-wheel/)</dct:source>
        <skos:definition xml:lang="en">a flavor that is musky or evocative of leather</skos:definition>
    </owl:Class>
    


    <!-- http://tw.rpi.edu/web/Courses/Ontologies/2016/OE_9_TeaTeam/AniseFlavor -->

    <owl:Class rdf:about="&tea;AniseFlavor">
        <rdfs:label xml:lang="en">anise flavor</rdfs:label>
        <rdfs:subClassOf rdf:resource="&tea;ASTASpiceFlavor"/>
        <rdfs:subClassOf rdf:resource="&tea;SpicyFlavor"/>
        <skos:definition>a flavor listed in the ASTA list that is reminiscent of anise, Pimpinella ansium</skos:definition>
        <dct:source>ASTA spice list (http://www.astaspice.org/download/9423/)</dct:source>
    </owl:Class>
    


    <!-- http://tw.rpi.edu/web/Courses/Ontologies/2016/OE_9_TeaTeam/ArilPart -->

    <owl:Class rdf:about="&tea;ArilPart">
        <rdfs:label xml:lang="en">aril plant part</rdfs:label>
        <rdfs:subClassOf rdf:resource="&tea;PlantPart"/>
        <rdfs:subClassOf>
            <owl:Restriction>
                <owl:onProperty rdf:resource="&tea;brewsAt"/>
                <owl:someValuesFrom rdf:resource="&tea;MediumBrewingTemperature"/>
            </owl:Restriction>
        </rdfs:subClassOf>
        <rdfs:subClassOf>
            <owl:Restriction>
                <owl:onProperty rdf:resource="&tea;brewsAt"/>
                <owl:someValuesFrom rdf:resource="&tea;LowBrewingTemperature"/>
            </owl:Restriction>
        </rdfs:subClassOf>
        <rdfs:subClassOf>
            <owl:Restriction>
                <owl:onProperty rdf:resource="&tea;brewsAt"/>
                <owl:someValuesFrom rdf:resource="&tea;HighBrewingTemperature"/>
            </owl:Restriction>
        </rdfs:subClassOf>
        <skos:definition>the aril of a plant, a growth that partially or fully covers a seed and may look like a fruit itself</skos:definition>
        <dct:source>Adapted from Merriam-Webster online dictionary</dct:source>
    </owl:Class>
    


    <!-- http://tw.rpi.edu/web/Courses/Ontologies/2016/OE_9_TeaTeam/BanchaGreenTea -->

    <owl:Class rdf:about="&tea;BanchaGreenTea">
        <rdfs:label xml:lang="en">bancha green tea</rdfs:label>
        <rdfs:subClassOf rdf:resource="&tea;GreenTea"/>
        <skos:definition>A green tea from Japan produced from unshaded steamed leaves that are picked in summer or autumn</skos:definition>
        <dct:source>http://infohost.nmt.edu/~armiller/japanese/tea.htm</dct:source>
        <skos:altLabel>番茶</skos:altLabel>
    </owl:Class>
    


    <!-- http://tw.rpi.edu/web/Courses/Ontologies/2016/OE_9_TeaTeam/BarkPart -->

    <owl:Class rdf:about="&tea;BarkPart">
        <rdfs:label xml:lang="en">bark part</rdfs:label>
        <rdfs:subClassOf rdf:resource="&tea;PlantPart"/>
        <rdfs:subClassOf>
            <owl:Restriction>
                <owl:onProperty rdf:resource="&tea;brewsAt"/>
                <owl:someValuesFrom rdf:resource="&tea;HighBrewingTemperature"/>
            </owl:Restriction>
        </rdfs:subClassOf>
        <dct:source>Adapted from Merriam-Webster online dictionary</dct:source>
        <skos:definition>the bark of a plant, the tough external covering of the stems or roots of woody plants</skos:definition>
    </owl:Class>
    


    <!-- http://tw.rpi.edu/web/Courses/Ontologies/2016/OE_9_TeaTeam/BasilFlavor -->

    <owl:Class rdf:about="&tea;BasilFlavor">
        <rdfs:label xml:lang="en">basil flavor</rdfs:label>
        <rdfs:subClassOf rdf:resource="&tea;ASTASpiceFlavor"/>
        <dct:source>ASTA spice list (http://www.astaspice.org/download/9423/)</dct:source>
        <skos:definition>a flavor listed in the ASTA list that is reminiscent of basil, the leaves of Ocimum basilicum</skos:definition>
    </owl:Class>
    


    <!-- http://tw.rpi.edu/web/Courses/Ontologies/2016/OE_9_TeaTeam/BayLeafFlavor -->

    <owl:Class rdf:about="&tea;BayLeafFlavor">
        <rdfs:label xml:lang="en">bay leaf flavor</rdfs:label>
        <rdfs:subClassOf rdf:resource="&tea;ASTASpiceFlavor"/>
        <rdfs:subClassOf rdf:resource="&tea;HerbalFlavor"/>
        <skos:definition>a flavor listed in the ASTA list that is reminiscent of bay leaves, a spice made from the leaves of one of several trees in the Lauraceae or Myrtaceae families</skos:definition>
        <dct:source>ASTA spice list (http://www.astaspice.org/download/9423/)</dct:source>
    </owl:Class>
    


    <!-- http://tw.rpi.edu/web/Courses/Ontologies/2016/OE_9_TeaTeam/BerryPart -->

    <owl:Class rdf:about="&tea;BerryPart">
        <rdfs:label xml:lang="en">berry part</rdfs:label>
        <rdfs:subClassOf rdf:resource="&tea;FruitPart"/>
        <skos:definition>culinarily, a fruit that is small and does not have a large seed within it, usually juicy</skos:definition>
        <dct:source>Adapted from Merriam-Webster online dictionary</dct:source>
    </owl:Class>
    


    <!-- http://tw.rpi.edu/web/Courses/Ontologies/2016/OE_9_TeaTeam/BitterFlavor -->

    <owl:Class rdf:about="&tea;BitterFlavor">
        <rdfs:label xml:lang="en">bitter flavor</rdfs:label>
        <rdfs:subClassOf rdf:resource="&tea;Flavor"/>
        <skos:definition xml:lang="en">a flavor that is acrid</skos:definition>
    </owl:Class>
    


    <!-- http://tw.rpi.edu/web/Courses/Ontologies/2016/OE_9_TeaTeam/BlackCarawayFlavor -->

    <owl:Class rdf:about="&tea;BlackCarawayFlavor">
        <rdfs:label xml:lang="en">black caraway flavor</rdfs:label>
        <rdfs:subClassOf rdf:resource="&tea;ASTASpiceFlavor"/>
        <rdfs:subClassOf rdf:resource="&tea;SpicyFlavor"/>
        <dct:source>ASTA spice list (http://www.astaspice.org/download/9423/)</dct:source>
        <skos:definition xml:lang="en">a flavor listed in the ASTA list that is reminiscent of black caraway, also known as black cumin, the seeds of the planf Nigella sativa</skos:definition>
    </owl:Class>
    


    <!-- http://tw.rpi.edu/web/Courses/Ontologies/2016/OE_9_TeaTeam/BlackPepperFlavor -->

    <owl:Class rdf:about="&tea;BlackPepperFlavor">
        <rdfs:label xml:lang="en">black pepper flavor</rdfs:label>
        <rdfs:subClassOf rdf:resource="&tea;ASTASpiceFlavor"/>
        <rdfs:subClassOf rdf:resource="&tea;SpicyFlavor"/>
        <dct:source>ASTA spice list (http://www.astaspice.org/download/9423/)</dct:source>
        <skos:definition>a flavor listed in the ASTA list that is reminiscent of black pepper, the dried fruits of the flowering vine Piper nigrum</skos:definition>
    </owl:Class>
    


    <!-- http://tw.rpi.edu/web/Courses/Ontologies/2016/OE_9_TeaTeam/BlackTea -->

    <owl:Class rdf:about="&tea;BlackTea">
        <rdfs:label xml:lang="en">black tea</rdfs:label>
        <rdfs:subClassOf rdf:resource="&tea;Tea"/>
        <skos:altLabel>紅茶</skos:altLabel>
        <dct:source>Tea: The Drink that Changed the World</dct:source>
        <skos:definition>Tea that has been withered, rolled, oxidized, and dried; completely oxidized</skos:definition>
    </owl:Class>
    


    <!-- http://tw.rpi.edu/web/Courses/Ontologies/2016/OE_9_TeaTeam/Blend -->

    <owl:Class rdf:about="&tea;Blend">
        <rdfs:label xml:lang="en">blend</rdfs:label>
        <owl:equivalentClass>
            <owl:Restriction>
                <owl:onProperty rdf:resource="&tea;contains"/>
                <owl:onClass rdf:resource="&tea;SteepedDrink"/>
                <owl:minQualifiedCardinality rdf:datatype="&xsd;nonNegativeInteger">2</owl:minQualifiedCardinality>
            </owl:Restriction>
        </owl:equivalentClass>
        <rdfs:subClassOf rdf:resource="&tea;DomainConcept"/>
        <dct:source>Merriam-Webster online dictionary</dct:source>
        <skos:definition>the combination of at least 2 steepedDrinks</skos:definition>
    </owl:Class>
    


    <!-- http://tw.rpi.edu/web/Courses/Ontologies/2016/OE_9_TeaTeam/BrewingTemperature -->

    <owl:Class rdf:about="&tea;BrewingTemperature">
        <rdfs:label xml:lang="en">brewing temperature</rdfs:label>
        <owl:equivalentClass>
            <owl:Class>
                <owl:unionOf rdf:parseType="Collection">
                    <rdf:Description rdf:about="&tea;HighBrewingTemperature"/>
                    <rdf:Description rdf:about="&tea;LowBrewingTemperature"/>
                    <rdf:Description rdf:about="&tea;MediumBrewingTemperature"/>
                </owl:unionOf>
            </owl:Class>
        </owl:equivalentClass>
        <rdfs:subClassOf rdf:resource="&tea;ValuePartition"/>
        <rdfs:subClassOf>
            <owl:Restriction>
                <owl:onProperty rdf:resource="&tea;brews"/>
                <owl:onClass rdf:resource="&tea;SteepedDrink"/>
                <owl:minQualifiedCardinality rdf:datatype="&xsd;nonNegativeInteger">1</owl:minQualifiedCardinality>
            </owl:Restriction>
        </rdfs:subClassOf>
        <dct:source>http://www.silkroadteas.com/how-to-brew-loose-leaf-tea-brewing-instructions/</dct:source>
        <skos:definition>The temperature of the water in which a steeped beverage is steeped</skos:definition>
    </owl:Class>
    


    <!-- http://tw.rpi.edu/web/Courses/Ontologies/2016/OE_9_TeaTeam/BudPart -->

    <owl:Class rdf:about="&tea;BudPart">
        <rdfs:label xml:lang="en">bud part</rdfs:label>
        <rdfs:subClassOf rdf:resource="&tea;FlowerPart"/>
        <skos:definition>an underdeveloped flower</skos:definition>
        <dct:source>Adapted from Merriam-Webster online dictionary</dct:source>
    </owl:Class>
    


    <!-- http://tw.rpi.edu/web/Courses/Ontologies/2016/OE_9_TeaTeam/Caffeinated -->

    <owl:Class rdf:about="&tea;Caffeinated">
        <rdfs:subClassOf rdf:resource="&tea;Caffeination"/>
        <owl:disjointWith rdf:resource="&tea;Decaffeinated"/>
        <skos:definition>Containing caffeine</skos:definition>
    </owl:Class>
    


    <!-- http://tw.rpi.edu/web/Courses/Ontologies/2016/OE_9_TeaTeam/CaffeinatedSteepedDrink -->

    <owl:Class rdf:about="&tea;CaffeinatedSteepedDrink">
        <rdfs:label xml:lang="en">caffeinated steeped drink</rdfs:label>
        <owl:equivalentClass>
            <owl:Class>
                <owl:intersectionOf rdf:parseType="Collection">
                    <rdf:Description rdf:about="&tea;SteepedDrink"/>
                    <owl:Restriction>
                        <owl:onProperty rdf:resource="&tea;hasCaffeine"/>
                        <owl:someValuesFrom rdf:resource="&tea;Caffeinated"/>
                    </owl:Restriction>
                </owl:intersectionOf>
            </owl:Class>
        </owl:equivalentClass>
        <rdfs:subClassOf rdf:resource="&tea;SteepedDrink"/>
        <owl:disjointWith rdf:resource="&tea;DecaffeinatedSteepedDrink"/>
        <skos:definition>a steeped drink that contains caffeine</skos:definition>
    </owl:Class>
    


    <!-- http://tw.rpi.edu/web/Courses/Ontologies/2016/OE_9_TeaTeam/Caffeination -->

    <owl:Class rdf:about="&tea;Caffeination">
        <rdfs:label xml:lang="en">caffeination</rdfs:label>
        <owl:equivalentClass>
            <owl:Class>
                <owl:unionOf rdf:parseType="Collection">
                    <rdf:Description rdf:about="&tea;Caffeinated"/>
                    <rdf:Description rdf:about="&tea;Decaffeinated"/>
                </owl:unionOf>
            </owl:Class>
        </owl:equivalentClass>
        <rdfs:subClassOf rdf:resource="&tea;ValuePartition"/>
        <skos:definition>Whether a brew has caffeine in it or not</skos:definition>
    </owl:Class>
    


    <!-- http://tw.rpi.edu/web/Courses/Ontologies/2016/OE_9_TeaTeam/CapsicumsFlavor -->

    <owl:Class rdf:about="&tea;CapsicumsFlavor">
        <rdfs:label xml:lang="en">capsicums flavor</rdfs:label>
        <rdfs:subClassOf rdf:resource="&tea;ASTASpiceFlavor"/>
        <rdfs:subClassOf rdf:resource="&tea;SpicyFlavor"/>
        <dct:source>ASTA spice list (http://www.astaspice.org/download/9423/)</dct:source>
        <skos:definition>a flavor listed in the ASTA list that is reminiscent of capsicums or peppers, the fruit of plants in the genus Capsicum</skos:definition>
    </owl:Class>
    


    <!-- http://tw.rpi.edu/web/Courses/Ontologies/2016/OE_9_TeaTeam/CarawaySeedFlavor -->

    <owl:Class rdf:about="&tea;CarawaySeedFlavor">
        <rdfs:label xml:lang="en">caraway seed flavor</rdfs:label>
        <rdfs:subClassOf rdf:resource="&tea;ASTASpiceFlavor"/>
        <rdfs:subClassOf rdf:resource="&tea;SpicyFlavor"/>
        <skos:definition>a flavor listed in the ASTA list that is reminiscent of caraway, the fruits of the plant Carum carvi</skos:definition>
        <dct:source>ASTA spice list (http://www.astaspice.org/download/9423/)</dct:source>
    </owl:Class>
    


    <!-- http://tw.rpi.edu/web/Courses/Ontologies/2016/OE_9_TeaTeam/CardamomFlavor -->

    <owl:Class rdf:about="&tea;CardamomFlavor">
        <rdfs:label xml:lang="en">cardamom flavor</rdfs:label>
        <rdfs:subClassOf rdf:resource="&tea;ASTASpiceFlavor"/>
        <rdfs:subClassOf rdf:resource="&tea;SpicyFlavor"/>
        <dct:source>ASTA spice list (http://www.astaspice.org/download/9423/)</dct:source>
        <skos:definition>a flavor listed in the ASTA list that is reminiscent of cardamom, the seeds of one of several plants in the Elettaria and Amomum genuses</skos:definition>
    </owl:Class>
    


    <!-- http://tw.rpi.edu/web/Courses/Ontologies/2016/OE_9_TeaTeam/CelerySeedFlavor -->

    <owl:Class rdf:about="&tea;CelerySeedFlavor">
        <rdfs:label xml:lang="en">celery seed flavor</rdfs:label>
        <rdfs:subClassOf rdf:resource="&tea;ASTASpiceFlavor"/>
        <rdfs:subClassOf rdf:resource="&tea;SpicyFlavor"/>
        <skos:definition>a flavor listed in the ASTA list that is reminiscent of celery seed, actually the fruit of the celery plant, Apium graveolens</skos:definition>
        <dct:source>ASTA spice list (http://www.astaspice.org/download/9423/)</dct:source>
    </owl:Class>
    


    <!-- http://tw.rpi.edu/web/Courses/Ontologies/2016/OE_9_TeaTeam/ChamomileFlavor -->

    <owl:Class rdf:about="&tea;ChamomileFlavor">
        <rdfs:label xml:lang="en">chamomile flavor</rdfs:label>
        <rdfs:subClassOf rdf:resource="&tea;ASTASpiceFlavor"/>
        <rdfs:subClassOf rdf:resource="&tea;FloralFlavor"/>
        <skos:definition>a flavor listed in the ASTA list that is reminiscent of chamomile, made from one of several species in the the family Asteraceae, most commonly Matricaria chamomilla or Chameamelum nobile</skos:definition>
        <dct:source>ASTA spice list (http://www.astaspice.org/download/9423/)</dct:source>
    </owl:Class>
    


    <!-- http://tw.rpi.edu/web/Courses/Ontologies/2016/OE_9_TeaTeam/ChervilFlavor -->

    <owl:Class rdf:about="&tea;ChervilFlavor">
        <rdfs:label xml:lang="en">chervil flavor</rdfs:label>
        <rdfs:subClassOf rdf:resource="&tea;ASTASpiceFlavor"/>
        <rdfs:subClassOf rdf:resource="&tea;HerbalFlavor"/>
        <dct:source>ASTA spice list (http://www.astaspice.org/download/9423/)</dct:source>
        <skos:definition>a flavor listed in the ASTA list that is reminiscent of chervil or French parsley, the plant Anthriscus cerefolium</skos:definition>
    </owl:Class>
    


    <!-- http://tw.rpi.edu/web/Courses/Ontologies/2016/OE_9_TeaTeam/ChiveFlavor -->

    <owl:Class rdf:about="&tea;ChiveFlavor">
        <rdfs:label xml:lang="en">chive flavor</rdfs:label>
        <rdfs:subClassOf rdf:resource="&tea;ASTASpiceFlavor"/>
        <rdfs:subClassOf rdf:resource="&tea;HerbalFlavor"/>
        <dct:source>ASTA spice list (http://www.astaspice.org/download/9423/)</dct:source>
        <skos:definition>a flavor listed in the ASTA list that is reminiscent of chive, the leaves of the plant Allium schoenoprasum</skos:definition>
    </owl:Class>
    


    <!-- http://tw.rpi.edu/web/Courses/Ontologies/2016/OE_9_TeaTeam/CilantroFlavor -->

    <owl:Class rdf:about="&tea;CilantroFlavor">
        <rdfs:label xml:lang="en">cilantro flavor</rdfs:label>
        <rdfs:subClassOf rdf:resource="&tea;ASTASpiceFlavor"/>
        <rdfs:subClassOf rdf:resource="&tea;HerbalFlavor"/>
        <skos:definition>a flavor listed in the ASTA list that is reminiscent of cilantro or coriander, the leaves of the plant Coriandrum sativum</skos:definition>
        <dct:source>ASTA spice list (http://www.astaspice.org/download/9423/)</dct:source>
    </owl:Class>
    


    <!-- http://tw.rpi.edu/web/Courses/Ontologies/2016/OE_9_TeaTeam/CinnamonFlavor -->

    <owl:Class rdf:about="&tea;CinnamonFlavor">
        <rdfs:label xml:lang="en">cinnamon flavor</rdfs:label>
        <rdfs:subClassOf rdf:resource="&tea;ASTASpiceFlavor"/>
        <rdfs:subClassOf rdf:resource="&tea;SpicyFlavor"/>
        <skos:definition>a flavor listed in the ASTA list that is reminiscent of cinnamon, the bark of one of several species in the Cinnamomum genus</skos:definition>
        <dct:source>ASTA spice list (http://www.astaspice.org/download/9423/)</dct:source>
    </owl:Class>
    


    <!-- http://tw.rpi.edu/web/Courses/Ontologies/2016/OE_9_TeaTeam/CloveFlavor -->

    <owl:Class rdf:about="&tea;CloveFlavor">
        <rdfs:label xml:lang="en">clove flavor</rdfs:label>
        <rdfs:subClassOf rdf:resource="&tea;ASTASpiceFlavor"/>
        <rdfs:subClassOf rdf:resource="&tea;SpicyFlavor"/>
        <skos:definition>a flavor listed in the ASTA list that is reminiscent of clove, the flower buds of the tree Syzygium aromaticum</skos:definition>
        <dct:source>ASTA spice list (http://www.astaspice.org/download/9423/)</dct:source>
    </owl:Class>
    


    <!-- http://tw.rpi.edu/web/Courses/Ontologies/2016/OE_9_TeaTeam/CompatibleBlend -->

    <owl:Class rdf:about="&tea;CompatibleBlend">
        <rdfs:label xml:lang="en">compatible blend</rdfs:label>
        <owl:equivalentClass>
            <owl:Restriction>
                <owl:onProperty rdf:resource="&tea;contains"/>
                <owl:someValuesFrom rdf:resource="&tea;FlavorCompatibility"/>
            </owl:Restriction>
        </owl:equivalentClass>
        <rdfs:subClassOf rdf:resource="&tea;Blend"/>
        <skos:definition>a blend of at least two drinks whose flavors are considered compatible</skos:definition>
    </owl:Class>
    


    <!-- http://tw.rpi.edu/web/Courses/Ontologies/2016/OE_9_TeaTeam/CorianderSeedFlavor -->

    <owl:Class rdf:about="&tea;CorianderSeedFlavor">
        <rdfs:label xml:lang="en">coriander flavor</rdfs:label>
        <rdfs:subClassOf rdf:resource="&tea;ASTASpiceFlavor"/>
        <rdfs:subClassOf rdf:resource="&tea;SpicyFlavor"/>
        <dct:source>ASTA spice list (http://www.astaspice.org/download/9423/)</dct:source>
        <skos:definition>a flavor listed in the ASTA list that is reminiscent of coriander seed, actually the fruits of the plant Coriandrum sativum</skos:definition>
    </owl:Class>
    


    <!-- http://tw.rpi.edu/web/Courses/Ontologies/2016/OE_9_TeaTeam/CuminSeedFlavor -->

    <owl:Class rdf:about="&tea;CuminSeedFlavor">
        <rdfs:label xml:lang="en">cumin seed flavor</rdfs:label>
        <rdfs:subClassOf rdf:resource="&tea;ASTASpiceFlavor"/>
        <rdfs:subClassOf rdf:resource="&tea;SpicyFlavor"/>
        <dct:source>ASTA spice list (http://www.astaspice.org/download/9423/)</dct:source>
        <skos:definition>a flavor listed in the ASTA list that is reminiscent of cumin, the seeds of the plant Cuminum cyminum</skos:definition>
    </owl:Class>
    


    <!-- http://tw.rpi.edu/web/Courses/Ontologies/2016/OE_9_TeaTeam/Decaffeinated -->

    <owl:Class rdf:about="&tea;Decaffeinated">
        <rdfs:subClassOf rdf:resource="&tea;Caffeination"/>
        <skos:definition>Not containing caffeine</skos:definition>
    </owl:Class>
    


    <!-- http://tw.rpi.edu/web/Courses/Ontologies/2016/OE_9_TeaTeam/DecaffeinatedBlend -->

    <owl:Class rdf:about="&tea;DecaffeinatedBlend">
        <rdfs:label xml:lang="en">decaffeinated blend</rdfs:label>
        <owl:equivalentClass>
            <owl:Restriction>
                <owl:onProperty rdf:resource="&tea;contains"/>
                <owl:allValuesFrom rdf:resource="&tea;DecaffeinatedSteepedDrink"/>
            </owl:Restriction>
        </owl:equivalentClass>
        <rdfs:subClassOf rdf:resource="&tea;Blend"/>
        <skos:definition>a blend which does not contain any steeped drinks that contain caffeine</skos:definition>
    </owl:Class>
    


    <!-- http://tw.rpi.edu/web/Courses/Ontologies/2016/OE_9_TeaTeam/DecaffeinatedSteepedDrink -->

    <owl:Class rdf:about="&tea;DecaffeinatedSteepedDrink">
        <rdfs:label xml:lang="en">decaffeinated steeped drink</rdfs:label>
        <owl:equivalentClass>
            <owl:Class>
                <owl:intersectionOf rdf:parseType="Collection">
                    <rdf:Description rdf:about="&tea;SteepedDrink"/>
                    <owl:Restriction>
                        <owl:onProperty rdf:resource="&tea;hasCaffeine"/>
                        <owl:allValuesFrom rdf:resource="&tea;Decaffeinated"/>
                    </owl:Restriction>
                </owl:intersectionOf>
            </owl:Class>
        </owl:equivalentClass>
        <rdfs:subClassOf rdf:resource="&tea;SteepedDrink"/>
        <skos:definition>a steeped drink which does not contain caffeine</skos:definition>
    </owl:Class>
    


    <!-- http://tw.rpi.edu/web/Courses/Ontologies/2016/OE_9_TeaTeam/DillSeedFlavor -->

    <owl:Class rdf:about="&tea;DillSeedFlavor">
        <rdfs:label xml:lang="en">dill seed flavor</rdfs:label>
        <rdfs:subClassOf rdf:resource="&tea;ASTASpiceFlavor"/>
        <rdfs:subClassOf rdf:resource="&tea;SpicyFlavor"/>
        <dct:source>ASTA spice list (http://www.astaspice.org/download/9423/)</dct:source>
        <skos:definition>a flavor listed in the ASTA list that is reminiscent of dill seed, the seed of the plant Anethum graveolens</skos:definition>
    </owl:Class>
    


    <!-- http://tw.rpi.edu/web/Courses/Ontologies/2016/OE_9_TeaTeam/DillWeedFlavor -->

    <owl:Class rdf:about="&tea;DillWeedFlavor">
        <rdfs:label xml:lang="en">dill weed flavor</rdfs:label>
        <rdfs:subClassOf rdf:resource="&tea;ASTASpiceFlavor"/>
        <rdfs:subClassOf rdf:resource="&tea;HerbalFlavor"/>
        <skos:definition>a flavor listed in the ASTA list that is reminiscent of dill weed, the leaves of the plant Anethum graveolens</skos:definition>
        <dct:source>ASTA spice list (http://www.astaspice.org/download/9423/)</dct:source>
    </owl:Class>
    


    <!-- http://tw.rpi.edu/web/Courses/Ontologies/2016/OE_9_TeaTeam/DomainConcept -->

    <owl:Class rdf:about="&tea;DomainConcept">
        <rdfs:label xml:lang="en">domain concept</rdfs:label>
        <owl:disjointWith rdf:resource="&tea;ValuePartition"/>
    </owl:Class>
    


    <!-- http://tw.rpi.edu/web/Courses/Ontologies/2016/OE_9_TeaTeam/EarthyFlavor -->

    <owl:Class rdf:about="&tea;EarthyFlavor">
        <rdfs:label xml:lang="en">earthy flavor</rdfs:label>
        <rdfs:subClassOf rdf:resource="&tea;Flavor"/>
        <dct:source>Adapted from Tea Cupping Standards (http://www.worldoftea.org/tea-cupping-standards/), Stone Leaf Tea&apos;s Tea Guru (http://www.stoneleaftea.com/tea-guru/), and The Australian Tea Maters&apos; Tea Flavour Wheel (https://australianteamasters.wordpress.com/2014/04/30/the-tea-flavour-wheel/)</dct:source>
        <skos:definition xml:lang="en">a flavor that is peaty or evocative of dirt or soil</skos:definition>
    </owl:Class>
    


    <!-- http://tw.rpi.edu/web/Courses/Ontologies/2016/OE_9_TeaTeam/FennelSeedFlavor -->

    <owl:Class rdf:about="&tea;FennelSeedFlavor">
        <rdfs:label xml:lang="en">fennel seed flavor</rdfs:label>
        <rdfs:subClassOf rdf:resource="&tea;ASTASpiceFlavor"/>
        <rdfs:subClassOf rdf:resource="&tea;SpicyFlavor"/>
        <skos:definition>a flavor listed in the ASTA list that is reminiscent of fennel, the seed of the flowering plant Foeniculum vulgare</skos:definition>
        <dct:source>ASTA spice list (http://www.astaspice.org/download/9423/)</dct:source>
    </owl:Class>
    


    <!-- http://tw.rpi.edu/web/Courses/Ontologies/2016/OE_9_TeaTeam/FenugreekSeedFlavor -->

    <owl:Class rdf:about="&tea;FenugreekSeedFlavor">
        <rdfs:label xml:lang="en">fenugreek seed flavor</rdfs:label>
        <rdfs:subClassOf rdf:resource="&tea;ASTASpiceFlavor"/>
        <rdfs:subClassOf rdf:resource="&tea;SpicyFlavor"/>
        <skos:definition>a flavor listed in the ASTA list that is reminiscent of fenugreek, the seeds of the plant Trigonella foenum-graecum</skos:definition>
        <dct:source>ASTA spice list (http://www.astaspice.org/download/9423/)</dct:source>
    </owl:Class>
    


    <!-- http://tw.rpi.edu/web/Courses/Ontologies/2016/OE_9_TeaTeam/Flavor -->

    <owl:Class rdf:about="&tea;Flavor">
        <rdfs:label xml:lang="en">flavor</rdfs:label>
        <rdfs:subClassOf rdf:resource="&tea;DomainConcept"/>
        <dct:source xml:lang="en">Merriam-Webster online dictionary</dct:source>
        <skos:definition xml:lang="en">the blend of taste and smell sensations evoked by a substance in the mouth</skos:definition>
    </owl:Class>
    


    <!-- http://tw.rpi.edu/web/Courses/Ontologies/2016/OE_9_TeaTeam/FlavorCompatibility -->

    <owl:Class rdf:about="&tea;FlavorCompatibility">
        <rdfs:label xml:lang="en">flavor compatibility</rdfs:label>
        <rdfs:subClassOf rdf:resource="&tea;DomainConcept"/>
        <skos:definition xml:lang="en">Two or more flavors deemed to be compatible by some source with some strength</skos:definition>
    </owl:Class>
    


    <!-- http://tw.rpi.edu/web/Courses/Ontologies/2016/OE_9_TeaTeam/FloralFlavor -->

    <owl:Class rdf:about="&tea;FloralFlavor">
        <rdfs:label xml:lang="en">floral flavor</rdfs:label>
        <rdfs:subClassOf rdf:resource="&tea;Flavor"/>
        <dct:source>Adapted from Tea Cupping Standards (http://www.worldoftea.org/tea-cupping-standards/), Stone Leaf Tea&apos;s Tea Guru (http://www.stoneleaftea.com/tea-guru/), and The Australian Tea Maters&apos; Tea Flavour Wheel (https://australianteamasters.wordpress.com/2014/04/30/the-tea-flavour-wheel/)</dct:source>
        <skos:definition xml:lang="en">a flavor that is evocative of flowers</skos:definition>
    </owl:Class>
    


    <!-- http://tw.rpi.edu/web/Courses/Ontologies/2016/OE_9_TeaTeam/FlowerPart -->

    <owl:Class rdf:about="&tea;FlowerPart">
        <rdfs:label xml:lang="en">flower part</rdfs:label>
        <rdfs:subClassOf rdf:resource="&tea;PlantPart"/>
        <rdfs:subClassOf>
            <owl:Restriction>
                <owl:onProperty rdf:resource="&tea;brewsAt"/>
                <owl:someValuesFrom rdf:resource="&tea;HighBrewingTemperature"/>
            </owl:Restriction>
        </rdfs:subClassOf>
        <rdfs:subClassOf>
            <owl:Restriction>
                <owl:onProperty rdf:resource="&tea;brewsAt"/>
                <owl:someValuesFrom rdf:resource="&tea;LowBrewingTemperature"/>
            </owl:Restriction>
        </rdfs:subClassOf>
        <rdfs:subClassOf>
            <owl:Restriction>
                <owl:onProperty rdf:resource="&tea;brewsAt"/>
                <owl:someValuesFrom rdf:resource="&tea;MediumBrewingTemperature"/>
            </owl:Restriction>
        </rdfs:subClassOf>
        <dct:source>Adapted from Merriam-Webster online dictionary</dct:source>
        <skos:definition>the flower of a plant, the reproductive structure of flowering plants</skos:definition>
    </owl:Class>
    


    <!-- http://tw.rpi.edu/web/Courses/Ontologies/2016/OE_9_TeaTeam/FruitPart -->

    <owl:Class rdf:about="&tea;FruitPart">
        <rdfs:label xml:lang="en">fruit part</rdfs:label>
        <rdfs:subClassOf rdf:resource="&tea;PlantPart"/>
        <rdfs:subClassOf>
            <owl:Restriction>
                <owl:onProperty rdf:resource="&tea;brewsAt"/>
                <owl:someValuesFrom rdf:resource="&tea;HighBrewingTemperature"/>
            </owl:Restriction>
        </rdfs:subClassOf>
        <skos:definition>the developed ovary of flowering plants</skos:definition>
        <dct:source>Adapted from Merriam-Webster online dictionary</dct:source>
    </owl:Class>
    


    <!-- http://tw.rpi.edu/web/Courses/Ontologies/2016/OE_9_TeaTeam/FruityFlavor -->

    <owl:Class rdf:about="&tea;FruityFlavor">
        <rdfs:label xml:lang="en">fruity flavor</rdfs:label>
        <rdfs:subClassOf rdf:resource="&tea;Flavor"/>
        <dct:source>Adapted from Tea Cupping Standards (http://www.worldoftea.org/tea-cupping-standards/), Stone Leaf Tea&apos;s Tea Guru (http://www.stoneleaftea.com/tea-guru/), and The Australian Tea Maters&apos; Tea Flavour Wheel (https://australianteamasters.wordpress.com/2014/04/30/the-tea-flavour-wheel/)</dct:source>
        <skos:definition xml:lang="en">a flavor that is evocative of fruit</skos:definition>
    </owl:Class>
    


    <!-- http://tw.rpi.edu/web/Courses/Ontologies/2016/OE_9_TeaTeam/GalangalFlavor -->

    <owl:Class rdf:about="&tea;GalangalFlavor">
        <rdfs:label xml:lang="en">galangal flavor</rdfs:label>
        <rdfs:subClassOf rdf:resource="&tea;ASTASpiceFlavor"/>
        <rdfs:subClassOf rdf:resource="&tea;SpicyFlavor"/>
        <dct:source>ASTA spice list (http://www.astaspice.org/download/9423/)</dct:source>
        <skos:definition>a flavor listed in the ASTA list that is reminiscent of galangal, the rhizome of one of several plants in the Zingiberaceae family</skos:definition>
    </owl:Class>
    


    <!-- http://tw.rpi.edu/web/Courses/Ontologies/2016/OE_9_TeaTeam/GingerFlavor -->

    <owl:Class rdf:about="&tea;GingerFlavor">
        <rdfs:label xml:lang="en">ginger flavor</rdfs:label>
        <rdfs:subClassOf rdf:resource="&tea;ASTASpiceFlavor"/>
        <rdfs:subClassOf rdf:resource="&tea;SpicyFlavor"/>
        <dct:source>ASTA spice list (http://www.astaspice.org/download/9423/)</dct:source>
        <skos:definition>a flavor listed in the ASTA list that is reminiscent of ginger, the rhizome of the flowering plant Zingiber officinale</skos:definition>
    </owl:Class>
    


    <!-- http://tw.rpi.edu/web/Courses/Ontologies/2016/OE_9_TeaTeam/GreenPeppercornFlavor -->

    <owl:Class rdf:about="&tea;GreenPeppercornFlavor">
        <rdfs:label xml:lang="en">green peppercorn flavor</rdfs:label>
        <rdfs:subClassOf rdf:resource="&tea;ASTASpiceFlavor"/>
        <rdfs:subClassOf rdf:resource="&tea;SpicyFlavor"/>
        <dct:source>ASTA spice list (http://www.astaspice.org/download/9423/)</dct:source>
        <skos:definition>a flavor listed in the ASTA list that is reminiscent of green pepper, the unripened seeds of the plant Piper nigrum that have been processed in a way that preserves their green color</skos:definition>
    </owl:Class>
    


    <!-- http://tw.rpi.edu/web/Courses/Ontologies/2016/OE_9_TeaTeam/GreenTea -->

    <owl:Class rdf:about="&tea;GreenTea">
        <rdfs:label xml:lang="en">green tea</rdfs:label>
        <rdfs:subClassOf rdf:resource="&tea;Tea"/>
        <rdfs:subClassOf>
            <owl:Restriction>
                <owl:onProperty rdf:resource="&tea;hasBrewingTemperature"/>
                <owl:someValuesFrom rdf:resource="&tea;LowBrewingTemperature"/>
            </owl:Restriction>
        </rdfs:subClassOf>
        <skos:altLabel>緑茶</skos:altLabel>
        <skos:definition>Tea that has been withered, rolled, and dried, but is not oxidized</skos:definition>
        <dct:source>Tea: The Drink that Changed the World</dct:source>
    </owl:Class>
    


    <!-- http://tw.rpi.edu/web/Courses/Ontologies/2016/OE_9_TeaTeam/Guayusa -->

    <owl:Class rdf:about="&tea;Guayusa">
        <rdfs:label xml:lang="en">guayusa</rdfs:label>
        <rdfs:subClassOf rdf:resource="&tea;CaffeinatedSteepedDrink"/>
        <rdfs:subClassOf rdf:resource="&tea;Tisane"/>
        <dct:source>http://runa.org/guayusa/</dct:source>
        <skos:definition>A steeped drink made from the leaves of Ilex guayusa, grown in South America. Contains caffeine.</skos:definition>
    </owl:Class>
    


    <!-- http://tw.rpi.edu/web/Courses/Ontologies/2016/OE_9_TeaTeam/GyokurochaGreenTea -->

    <owl:Class rdf:about="&tea;GyokurochaGreenTea">
        <rdfs:label xml:lang="en">gyokurocha green tea</rdfs:label>
        <rdfs:subClassOf rdf:resource="&tea;GreenTea"/>
        <skos:definition>A green tea from Japan produced from steamed leaves that were shaded during growth</skos:definition>
        <skos:altLabel>玉露茶</skos:altLabel>
        <dct:source>http://infohost.nmt.edu/~armiller/japanese/tea.htm</dct:source>
    </owl:Class>
    


    <!-- http://tw.rpi.edu/web/Courses/Ontologies/2016/OE_9_TeaTeam/HerbalFlavor -->

    <owl:Class rdf:about="&tea;HerbalFlavor">
        <rdfs:label xml:lang="en">herbal flavor</rdfs:label>
        <rdfs:subClassOf rdf:resource="&tea;Flavor"/>
        <dct:source>Adapted from Foy Spicer, Department of Horticulture, Iowa State University, in Horticulture and Home Pest News, IC-489(21) -- August 22, 2003</dct:source>
        <skos:definition xml:lang="en">a flavor that is evocative of culinary/medicinal herbs - leaves of plants used for savory or medicinal purposes</skos:definition>
    </owl:Class>
    


    <!-- http://tw.rpi.edu/web/Courses/Ontologies/2016/OE_9_TeaTeam/HighBrewingTemperature -->

    <owl:Class rdf:about="&tea;HighBrewingTemperature">
        <rdfs:label xml:lang="en">high brewing temperature</rdfs:label>
        <rdfs:subClassOf rdf:resource="&tea;BrewingTemperature"/>
        <owl:disjointWith rdf:resource="&tea;LowBrewingTemperature"/>
        <owl:disjointWith rdf:resource="&tea;MediumBrewingTemperature"/>
        <dct:source>http://www.silkroadteas.com/how-to-brew-loose-leaf-tea-brewing-instructions/</dct:source>
        <skos:definition>205~212°F or 96~100°C</skos:definition>
    </owl:Class>
    


    <!-- http://tw.rpi.edu/web/Courses/Ontologies/2016/OE_9_TeaTeam/HorseradishFlavor -->

    <owl:Class rdf:about="&tea;HorseradishFlavor">
        <rdfs:label xml:lang="en">horseradish flavor</rdfs:label>
        <rdfs:subClassOf rdf:resource="&tea;ASTASpiceFlavor"/>
        <rdfs:subClassOf rdf:resource="&tea;SpicyFlavor"/>
        <dct:source>ASTA spice list (http://www.astaspice.org/download/9423/)</dct:source>
        <skos:definition>a flavor listed in the ASTA list that is reminiscent of horseradish, the root of the plant Armoracia rusticana</skos:definition>
    </owl:Class>
    


    <!-- http://tw.rpi.edu/web/Courses/Ontologies/2016/OE_9_TeaTeam/HoujichaGreenTea -->

    <owl:Class rdf:about="&tea;HoujichaGreenTea">
        <rdfs:label xml:lang="en">houjicha green tea</rdfs:label>
        <rdfs:subClassOf rdf:resource="&tea;GreenTea"/>
        <skos:altLabel>ほうじ茶</skos:altLabel>
        <skos:definition>A green tea from Japan produced from unshaded leaves that are roasted rather than steamed</skos:definition>
        <dct:source>http://infohost.nmt.edu/~armiller/japanese/tea.htm</dct:source>
    </owl:Class>
    


    <!-- http://tw.rpi.edu/web/Courses/Ontologies/2016/OE_9_TeaTeam/JuniperFlavor -->

    <owl:Class rdf:about="&tea;JuniperFlavor">
        <rdfs:label xml:lang="en">juniper flavor</rdfs:label>
        <rdfs:subClassOf rdf:resource="&tea;ASTASpiceFlavor"/>
        <rdfs:subClassOf rdf:resource="&tea;SpicyFlavor"/>
        <skos:definition>a flavor listed in the ASTA list that is reminiscent of juniper berries, from the trees in the genus Juniperus</skos:definition>
        <dct:source>ASTA spice list (http://www.astaspice.org/download/9423/)</dct:source>
    </owl:Class>
    


    <!-- http://tw.rpi.edu/web/Courses/Ontologies/2016/OE_9_TeaTeam/KabusechaGreenTea -->

    <owl:Class rdf:about="&tea;KabusechaGreenTea">
        <rdfs:label xml:lang="en">kabusecha green tea</rdfs:label>
        <rdfs:subClassOf rdf:resource="&tea;GreenTea"/>
        <skos:definition>A green tea from Japan produced from steamed leaves that were shaded during part of the last part of growth before harvest</skos:definition>
        <dct:source>http://infohost.nmt.edu/~armiller/japanese/tea.htm</dct:source>
        <skos:altLabel>かぶせ茶</skos:altLabel>
    </owl:Class>
    


    <!-- http://tw.rpi.edu/web/Courses/Ontologies/2016/OE_9_TeaTeam/LavenderFlavor -->

    <owl:Class rdf:about="&tea;LavenderFlavor">
        <rdfs:label xml:lang="en">lavender flavor</rdfs:label>
        <rdfs:subClassOf rdf:resource="&tea;ASTASpiceFlavor"/>
        <rdfs:subClassOf rdf:resource="&tea;FloralFlavor"/>
        <dct:source>ASTA spice list (http://www.astaspice.org/download/9423/)</dct:source>
        <skos:definition>a flavor listed in the ASTA list that is reminiscent of lavender, the flowers of the plant Lavandula angustifolia</skos:definition>
    </owl:Class>
    


    <!-- http://tw.rpi.edu/web/Courses/Ontologies/2016/OE_9_TeaTeam/LeafPart -->

    <owl:Class rdf:about="&tea;LeafPart">
        <rdfs:label xml:lang="en">leaf part</rdfs:label>
        <rdfs:subClassOf rdf:resource="&tea;PlantPart"/>
        <rdfs:subClassOf>
            <owl:Restriction>
                <owl:onProperty rdf:resource="&tea;brewsAt"/>
                <owl:someValuesFrom rdf:resource="&tea;MediumBrewingTemperature"/>
            </owl:Restriction>
        </rdfs:subClassOf>
        <rdfs:subClassOf>
            <owl:Restriction>
                <owl:onProperty rdf:resource="&tea;brewsAt"/>
                <owl:someValuesFrom rdf:resource="&tea;HighBrewingTemperature"/>
            </owl:Restriction>
        </rdfs:subClassOf>
        <rdfs:subClassOf>
            <owl:Restriction>
                <owl:onProperty rdf:resource="&tea;brewsAt"/>
                <owl:someValuesFrom rdf:resource="&tea;LowBrewingTemperature"/>
            </owl:Restriction>
        </rdfs:subClassOf>
        <skos:definition>the structure used by a plant to perform photosynthesis</skos:definition>
        <dct:source>Adapted from Merriam-Webster online dictionary</dct:source>
    </owl:Class>
    


    <!-- http://tw.rpi.edu/web/Courses/Ontologies/2016/OE_9_TeaTeam/LemonBalmFlavor -->

    <owl:Class rdf:about="&tea;LemonBalmFlavor">
        <rdfs:label xml:lang="en">lemon balm flavor</rdfs:label>
        <rdfs:subClassOf rdf:resource="&tea;ASTASpiceFlavor"/>
        <rdfs:subClassOf rdf:resource="&tea;HerbalFlavor"/>
        <skos:definition>a flavor listed in the ASTA list that is reminiscent of lemon balm, the leaves of the plant Melissa officinalis</skos:definition>
        <dct:source>ASTA spice list (http://www.astaspice.org/download/9423/)</dct:source>
    </owl:Class>
    


    <!-- http://tw.rpi.edu/web/Courses/Ontologies/2016/OE_9_TeaTeam/LowBrewingTemperature -->

    <owl:Class rdf:about="&tea;LowBrewingTemperature">
        <rdfs:label xml:lang="en">low brewing temperature</rdfs:label>
        <rdfs:subClassOf rdf:resource="&tea;BrewingTemperature"/>
        <owl:disjointWith rdf:resource="&tea;MediumBrewingTemperature"/>
        <skos:definition>160~185°F or 71~85°C</skos:definition>
        <dct:source>http://www.silkroadteas.com/how-to-brew-loose-leaf-tea-brewing-instructions/</dct:source>
    </owl:Class>
    


    <!-- http://tw.rpi.edu/web/Courses/Ontologies/2016/OE_9_TeaTeam/MacchaGreenTea -->

    <owl:Class rdf:about="&tea;MacchaGreenTea">
        <rdfs:label xml:lang="en">maccha green tea</rdfs:label>
        <rdfs:subClassOf rdf:resource="&tea;GreenTea"/>
        <skos:definition>A green tea from Japan produced from steamed leaves that were shaded during growth, then powdered after drying.</skos:definition>
        <dct:source>http://infohost.nmt.edu/~armiller/japanese/tea.htm</dct:source>
        <skos:altLabel xml:lang="en">matcha green tea</skos:altLabel>
        <skos:altLabel>抹茶</skos:altLabel>
    </owl:Class>
    


    <!-- http://tw.rpi.edu/web/Courses/Ontologies/2016/OE_9_TeaTeam/MaceFlavor -->

    <owl:Class rdf:about="&tea;MaceFlavor">
        <rdfs:label xml:lang="en">mace flavor</rdfs:label>
        <rdfs:subClassOf rdf:resource="&tea;ASTASpiceFlavor"/>
        <rdfs:subClassOf rdf:resource="&tea;SpicyFlavor"/>
        <dct:source>ASTA spice list (http://www.astaspice.org/download/9423/)</dct:source>
        <skos:definition>a flavor listed in the ASTA list that is reminiscent of mace, the dried covering or aril of the nutmeg seed, in one of several species in the genus Myristica</skos:definition>
    </owl:Class>
    


    <!-- http://tw.rpi.edu/web/Courses/Ontologies/2016/OE_9_TeaTeam/MajoramLeafFlavor -->

    <owl:Class rdf:about="&tea;MajoramLeafFlavor">
        <rdfs:label xml:lang="en">majoram leaf flavor</rdfs:label>
        <rdfs:subClassOf rdf:resource="&tea;ASTASpiceFlavor"/>
        <rdfs:subClassOf rdf:resource="&tea;HerbalFlavor"/>
        <skos:definition>a flavor listed in the ASTA list that is reminiscent of majorum, the leaves of the herb Origanum majorana</skos:definition>
        <dct:source>ASTA spice list (http://www.astaspice.org/download/9423/)</dct:source>
    </owl:Class>
    


    <!-- http://tw.rpi.edu/web/Courses/Ontologies/2016/OE_9_TeaTeam/MarineFlavor -->

    <owl:Class rdf:about="&tea;MarineFlavor">
        <rdfs:label xml:lang="en">marine flavor</rdfs:label>
        <rdfs:subClassOf rdf:resource="&tea;Flavor"/>
        <dct:source>Adapted from Tea Cupping Standards (http://www.worldoftea.org/tea-cupping-standards/), Stone Leaf Tea&apos;s Tea Guru (http://www.stoneleaftea.com/tea-guru/), and The Australian Tea Maters&apos; Tea Flavour Wheel (https://australianteamasters.wordpress.com/2014/04/30/the-tea-flavour-wheel/)</dct:source>
        <skos:definition xml:lang="en">a flavor that is salty, fishy, or evocative of the sea</skos:definition>
    </owl:Class>
    


    <!-- http://tw.rpi.edu/web/Courses/Ontologies/2016/OE_9_TeaTeam/MediumBrewingTemperature -->

    <owl:Class rdf:about="&tea;MediumBrewingTemperature">
        <rdfs:label xml:lang="en">medium brewing temperature</rdfs:label>
        <rdfs:subClassOf rdf:resource="&tea;BrewingTemperature"/>
        <skos:definition>185~205°F or 85~96°C</skos:definition>
        <dct:source>http://www.silkroadteas.com/how-to-brew-loose-leaf-tea-brewing-instructions/</dct:source>
    </owl:Class>
    


    <!-- http://tw.rpi.edu/web/Courses/Ontologies/2016/OE_9_TeaTeam/MintTea -->

    <owl:Class rdf:about="&tea;MintTea">
        <rdfs:label xml:lang="en">mint tea</rdfs:label>
        <rdfs:subClassOf rdf:resource="&tea;DecaffeinatedSteepedDrink"/>
        <rdfs:subClassOf rdf:resource="&tea;Tisane"/>
        <rdfs:subClassOf>
            <owl:Restriction>
                <owl:onProperty rdf:resource="&tea;madeFromPart"/>
                <owl:someValuesFrom rdf:resource="&tea;LeafPart"/>
            </owl:Restriction>
        </rdfs:subClassOf>
        <dct:source>Wikipedia</dct:source>
        <skos:definition>a tisane made from the leaves of plants in the Mentha family</skos:definition>
    </owl:Class>
    


    <!-- http://tw.rpi.edu/web/Courses/Ontologies/2016/OE_9_TeaTeam/MustardSeedFlavor -->

    <owl:Class rdf:about="&tea;MustardSeedFlavor">
        <rdfs:label xml:lang="en">mustard seed flavor</rdfs:label>
        <rdfs:subClassOf rdf:resource="&tea;ASTASpiceFlavor"/>
        <rdfs:subClassOf rdf:resource="&tea;SpicyFlavor"/>
        <dct:source>ASTA spice list (http://www.astaspice.org/download/9423/)</dct:source>
        <skos:definition>a flavor listed in the ASTA list that is reminiscent of mustard seed, the seed of either Brassica nigra, Brassica juncea, or Brassica alba/Sinapis alba</skos:definition>
    </owl:Class>
    


    <!-- http://tw.rpi.edu/web/Courses/Ontologies/2016/OE_9_TeaTeam/NutmegFlavor -->

    <owl:Class rdf:about="&tea;NutmegFlavor">
        <rdfs:label xml:lang="en">nutmeg flavor</rdfs:label>
        <rdfs:subClassOf rdf:resource="&tea;ASTASpiceFlavor"/>
        <rdfs:subClassOf rdf:resource="&tea;SpicyFlavor"/>
        <skos:definition>a flavor listed in the ASTA list that is reminiscent of nutmeg, the seed of the nutmeg tree, from one of several species in the genus Myristica</skos:definition>
        <dct:source>ASTA spice list (http://www.astaspice.org/download/9423/)</dct:source>
    </owl:Class>
    


    <!-- http://tw.rpi.edu/web/Courses/Ontologies/2016/OE_9_TeaTeam/NuttyFlavor -->

    <owl:Class rdf:about="&tea;NuttyFlavor">
        <rdfs:label xml:lang="en">nutty flavor</rdfs:label>
        <rdfs:subClassOf rdf:resource="&tea;Flavor"/>
        <dct:source>Adapted from Tea Cupping Standards (http://www.worldoftea.org/tea-cupping-standards/), Stone Leaf Tea&apos;s Tea Guru (http://www.stoneleaftea.com/tea-guru/), and The Australian Tea Maters&apos; Tea Flavour Wheel (https://australianteamasters.wordpress.com/2014/04/30/the-tea-flavour-wheel/)</dct:source>
        <skos:definition xml:lang="en">a flavor that is evocative of nuts</skos:definition>
    </owl:Class>
    


    <!-- http://tw.rpi.edu/web/Courses/Ontologies/2016/OE_9_TeaTeam/OolongTea -->

    <owl:Class rdf:about="&tea;OolongTea">
        <rdfs:label xml:lang="en">oolong tea</rdfs:label>
        <rdfs:subClassOf rdf:resource="&tea;Tea"/>
        <skos:definition>Tea that has been withered, rolled, oxidized, and dried; partially but not completely oxidized</skos:definition>
        <dct:source>Tea: The Drink that Changed the World</dct:source>
        <skos:altLabel>烏龍茶</skos:altLabel>
    </owl:Class>
    


    <!-- http://tw.rpi.edu/web/Courses/Ontologies/2016/OE_9_TeaTeam/OreganoLeafFlavor -->

    <owl:Class rdf:about="&tea;OreganoLeafFlavor">
        <rdfs:label xml:lang="en">oregano flavor</rdfs:label>
        <rdfs:subClassOf rdf:resource="&tea;ASTASpiceFlavor"/>
        <rdfs:subClassOf rdf:resource="&tea;HerbalFlavor"/>
        <dct:source>ASTA spice list (http://www.astaspice.org/download/9423/)</dct:source>
        <skos:definition>a flavor listed in the ASTA list that is reminiscent of oregano, the leaves of Origanum vulgare</skos:definition>
    </owl:Class>
    


    <!-- http://tw.rpi.edu/web/Courses/Ontologies/2016/OE_9_TeaTeam/PaprikaFlavor -->

    <owl:Class rdf:about="&tea;PaprikaFlavor">
        <rdfs:label xml:lang="en">paprika flavor</rdfs:label>
        <rdfs:subClassOf rdf:resource="&tea;ASTASpiceFlavor"/>
        <rdfs:subClassOf rdf:resource="&tea;SpicyFlavor"/>
        <dct:source>ASTA spice list (http://www.astaspice.org/download/9423/)</dct:source>
        <skos:definition>a flavor listed in the ASTA list that is reminiscent of paprika, the dried fruit of the plant Capsicum annuum</skos:definition>
    </owl:Class>
    


    <!-- http://tw.rpi.edu/web/Courses/Ontologies/2016/OE_9_TeaTeam/ParsleyFlavor -->

    <owl:Class rdf:about="&tea;ParsleyFlavor">
        <rdfs:label xml:lang="en">parsley flavor</rdfs:label>
        <rdfs:subClassOf rdf:resource="&tea;ASTASpiceFlavor"/>
        <rdfs:subClassOf rdf:resource="&tea;HerbalFlavor"/>
        <dct:source>ASTA spice list (http://www.astaspice.org/download/9423/)</dct:source>
        <skos:definition>a flavor listed in the ASTA list that is reminiscent of parsley, the leaves of the plant Petroselinum crispum</skos:definition>
    </owl:Class>
    


    <!-- http://tw.rpi.edu/web/Courses/Ontologies/2016/OE_9_TeaTeam/PeppermintLeafFlavor -->

    <owl:Class rdf:about="&tea;PeppermintLeafFlavor">
        <rdfs:label xml:lang="en">pepperment leaf flavor</rdfs:label>
        <rdfs:subClassOf rdf:resource="&tea;ASTASpiceFlavor"/>
        <rdfs:subClassOf rdf:resource="&tea;HerbalFlavor"/>
        <dct:source>ASTA spice list (http://www.astaspice.org/download/9423/)</dct:source>
        <skos:definition>a flavor listed in the ASTA list that is reminiscent of peppermint, the leaves of Mentha x piperita, a hybrid between Mentha aquatica and Mentha spicata</skos:definition>
    </owl:Class>
    


    <!-- http://tw.rpi.edu/web/Courses/Ontologies/2016/OE_9_TeaTeam/PinkPeppercornFlavor -->

    <owl:Class rdf:about="&tea;PinkPeppercornFlavor">
        <rdfs:label xml:lang="en">pink peppercorn flavor</rdfs:label>
        <rdfs:subClassOf rdf:resource="&tea;ASTASpiceFlavor"/>
        <rdfs:subClassOf rdf:resource="&tea;SpicyFlavor"/>
        <dct:source>ASTA spice list (http://www.astaspice.org/download/9423/)</dct:source>
        <skos:definition>a flavor listed in the ASTA list that is reminiscent of pink peppercorn, the dried berry of the shrub Schinus molle</skos:definition>
    </owl:Class>
    


    <!-- http://tw.rpi.edu/web/Courses/Ontologies/2016/OE_9_TeaTeam/PlantPart -->

    <owl:Class rdf:about="&tea;PlantPart">
        <rdfs:label xml:lang="en">plant part</rdfs:label>
        <rdfs:subClassOf rdf:resource="&tea;DomainConcept"/>
        <skos:definition xml:lang="en">a part of a plant, defined culinarily, not botanically</skos:definition>
    </owl:Class>
    


    <!-- http://tw.rpi.edu/web/Courses/Ontologies/2016/OE_9_TeaTeam/PoppySeedFlavor -->

    <owl:Class rdf:about="&tea;PoppySeedFlavor">
        <rdfs:label xml:lang="en">poppy seed flavor</rdfs:label>
        <rdfs:subClassOf rdf:resource="&tea;ASTASpiceFlavor"/>
        <rdfs:subClassOf rdf:resource="&tea;SpicyFlavor"/>
        <skos:definition>a flavor listed in the ASTA list that is reminiscent of poppy seed, the seed of the flower Papaver somniferum</skos:definition>
        <dct:source>ASTA spice list (http://www.astaspice.org/download/9423/)</dct:source>
    </owl:Class>
    


    <!-- http://tw.rpi.edu/web/Courses/Ontologies/2016/OE_9_TeaTeam/Pu-ErhTea -->

    <owl:Class rdf:about="&tea;Pu-ErhTea">
        <rdfs:label xml:lang="en">pu-erh tea</rdfs:label>
        <rdfs:subClassOf rdf:resource="&tea;Tea"/>
        <dct:source>Tea: The Drink that Changed the World</dct:source>
        <skos:altLabel>普洱茶</skos:altLabel>
        <skos:definition>Tea that is fermented, made from large tea leaves from older plants</skos:definition>
    </owl:Class>
    


    <!-- http://tw.rpi.edu/web/Courses/Ontologies/2016/OE_9_TeaTeam/RipePu-ErhTea -->

    <owl:Class rdf:about="&tea;RipePu-ErhTea">
        <rdfs:label xml:lang="en">ripe pu-erh tea</rdfs:label>
        <rdfs:subClassOf rdf:resource="&tea;Pu-ErhTea"/>
        <rdfs:subClassOf>
            <owl:Restriction>
                <owl:onProperty rdf:resource="&tea;hasBrewingTemperature"/>
                <owl:someValuesFrom rdf:resource="&tea;HighBrewingTemperature"/>
            </owl:Restriction>
        </rdfs:subClassOf>
        <skos:definition>A pu-erh tea that is piled and left to ferment after processing</skos:definition>
        <dct:source>http://www.seriouseats.com/2015/08/what-is-puerh-tea-where-to-buy.html</dct:source>
    </owl:Class>
    


    <!-- http://tw.rpi.edu/web/Courses/Ontologies/2016/OE_9_TeaTeam/RooibosTea -->

    <owl:Class rdf:about="&tea;RooibosTea">
        <rdfs:label xml:lang="en">rooibos tea</rdfs:label>
        <rdfs:subClassOf rdf:resource="&tea;DecaffeinatedSteepedDrink"/>
        <rdfs:subClassOf rdf:resource="&tea;Tisane"/>
        <dct:source>Tea: The Drink that Changed the World</dct:source>
        <skos:definition>A steeped drink made from the leaves of Aspalanthus linearis, grown in South Africa. Contains no caffeine.</skos:definition>
        <skos:altLabel xml:lang="en">red tea</skos:altLabel>
    </owl:Class>
    


    <!-- http://tw.rpi.edu/web/Courses/Ontologies/2016/OE_9_TeaTeam/RootPart -->

    <owl:Class rdf:about="&tea;RootPart">
        <rdfs:label xml:lang="en">root part</rdfs:label>
        <rdfs:subClassOf rdf:resource="&tea;PlantPart"/>
        <rdfs:subClassOf>
            <owl:Restriction>
                <owl:onProperty rdf:resource="&tea;brewsAt"/>
                <owl:someValuesFrom rdf:resource="&tea;HighBrewingTemperature"/>
            </owl:Restriction>
        </rdfs:subClassOf>
        <skos:definition>an underground part of a plant, used for gathering nutrients, storing nutrients, or for supporting the plant</skos:definition>
        <dct:source>Adapted from Merriam-Webster online dictionary</dct:source>
    </owl:Class>
    


    <!-- http://tw.rpi.edu/web/Courses/Ontologies/2016/OE_9_TeaTeam/RosemaryFlavor -->

    <owl:Class rdf:about="&tea;RosemaryFlavor">
        <rdfs:label xml:lang="en">rosemary flavor</rdfs:label>
        <rdfs:subClassOf rdf:resource="&tea;ASTASpiceFlavor"/>
        <rdfs:subClassOf rdf:resource="&tea;HerbalFlavor"/>
        <dct:source>ASTA spice list (http://www.astaspice.org/download/9423/)</dct:source>
        <skos:definition>a flavor listed in the ASTA list that is reminiscent of rosemary, the leaves of the herb Rosmarinus officinalis</skos:definition>
    </owl:Class>
    


    <!-- http://tw.rpi.edu/web/Courses/Ontologies/2016/OE_9_TeaTeam/SageFlavor -->

    <owl:Class rdf:about="&tea;SageFlavor">
        <rdfs:label xml:lang="en">sage flavor</rdfs:label>
        <rdfs:subClassOf rdf:resource="&tea;ASTASpiceFlavor"/>
        <rdfs:subClassOf rdf:resource="&tea;HerbalFlavor"/>
        <skos:definition>a flavor listed in the ASTA list that is reminiscent of sage, the leaves of the plant Salvia officinalis</skos:definition>
        <dct:source>ASTA spice list (http://www.astaspice.org/download/9423/)</dct:source>
    </owl:Class>
    


    <!-- http://tw.rpi.edu/web/Courses/Ontologies/2016/OE_9_TeaTeam/SavoryLeafFlavor -->

    <owl:Class rdf:about="&tea;SavoryLeafFlavor">
        <rdfs:label xml:lang="en">savory leaf flavor</rdfs:label>
        <rdfs:subClassOf rdf:resource="&tea;ASTASpiceFlavor"/>
        <rdfs:subClassOf rdf:resource="&tea;HerbalFlavor"/>
        <dct:source>ASTA spice list (http://www.astaspice.org/download/9423/)</dct:source>
        <skos:definition>a flavor listed in the ASTA list that is reminiscent of savory, the leaves of the plant Satureja hortensis or Satureja montana</skos:definition>
    </owl:Class>
    


    <!-- http://tw.rpi.edu/web/Courses/Ontologies/2016/OE_9_TeaTeam/SeedPart -->

    <owl:Class rdf:about="&tea;SeedPart">
        <rdfs:label xml:lang="en">seed part</rdfs:label>
        <rdfs:subClassOf rdf:resource="&tea;PlantPart"/>
        <rdfs:subClassOf>
            <owl:Restriction>
                <owl:onProperty rdf:resource="&tea;brewsAt"/>
                <owl:someValuesFrom rdf:resource="&tea;HighBrewingTemperature"/>
            </owl:Restriction>
        </rdfs:subClassOf>
        <skos:definition>the developed, fertilized part of a flowering plant</skos:definition>
        <dct:source>Adapted from Merriam-Webster online dictionary</dct:source>
    </owl:Class>
    


    <!-- http://tw.rpi.edu/web/Courses/Ontologies/2016/OE_9_TeaTeam/SenchaGreenTea -->

    <owl:Class rdf:about="&tea;SenchaGreenTea">
        <rdfs:label xml:lang="en">sencha green tea</rdfs:label>
        <rdfs:subClassOf rdf:resource="&tea;GreenTea"/>
        <skos:definition>A green tea from Japan produced from unshaded steamed leaves picked during spring</skos:definition>
        <dct:source>http://infohost.nmt.edu/~armiller/japanese/tea.htm</dct:source>
        <skos:altLabel>煎茶</skos:altLabel>
    </owl:Class>
    


    <!-- http://tw.rpi.edu/web/Courses/Ontologies/2016/OE_9_TeaTeam/SesameSeedFlavor -->

    <owl:Class rdf:about="&tea;SesameSeedFlavor">
        <rdfs:label xml:lang="en">sesame seed flavor</rdfs:label>
        <rdfs:subClassOf rdf:resource="&tea;ASTASpiceFlavor"/>
        <rdfs:subClassOf rdf:resource="&tea;SpicyFlavor"/>
        <skos:definition>a flavor listed in the ASTA list that is reminiscent of sesame seed, the seed of the plant Sesamum indicum</skos:definition>
        <dct:source>ASTA spice list (http://www.astaspice.org/download/9423/)</dct:source>
    </owl:Class>
    


    <!-- http://tw.rpi.edu/web/Courses/Ontologies/2016/OE_9_TeaTeam/SourFlavor -->

    <owl:Class rdf:about="&tea;SourFlavor">
        <rdfs:label xml:lang="en">sour flavor</rdfs:label>
        <rdfs:subClassOf rdf:resource="&tea;Flavor"/>
        <skos:definition xml:lang="en">a flavor that is tart or acidic</skos:definition>
    </owl:Class>
    


    <!-- http://tw.rpi.edu/web/Courses/Ontologies/2016/OE_9_TeaTeam/SpearmintFlavor -->

    <owl:Class rdf:about="&tea;SpearmintFlavor">
        <rdfs:label xml:lang="en">spearmint flavor</rdfs:label>
        <rdfs:subClassOf rdf:resource="&tea;ASTASpiceFlavor"/>
        <rdfs:subClassOf rdf:resource="&tea;HerbalFlavor"/>
        <dct:source>ASTA spice list (http://www.astaspice.org/download/9423/)</dct:source>
        <skos:definition>a flavor listed in the ASTA list that is reminiscent of spearmint, the leaves of the plant Mentha spicata</skos:definition>
    </owl:Class>
    


    <!-- http://tw.rpi.edu/web/Courses/Ontologies/2016/OE_9_TeaTeam/SpicyFlavor -->

    <owl:Class rdf:about="&tea;SpicyFlavor">
        <rdfs:label xml:lang="en">spicy flavor</rdfs:label>
        <rdfs:subClassOf rdf:resource="&tea;Flavor"/>
        <dct:source>Adapted from Foy Spicer, Department of Horticulture, Iowa State University, in Horticulture and Home Pest News, IC-489(21) -- August 22, 2003</dct:source>
        <skos:definition xml:lang="en">a flavor that is evocative of culinary/medicinal spices - aromatic substances obtained from roots, flowers, fruits, seeds or bark; not necessarily capsaicin</skos:definition>
    </owl:Class>
    


    <!-- http://tw.rpi.edu/web/Courses/Ontologies/2016/OE_9_TeaTeam/StarAniseFlavor -->

    <owl:Class rdf:about="&tea;StarAniseFlavor">
        <rdfs:label xml:lang="en">star anise flavor</rdfs:label>
        <rdfs:subClassOf rdf:resource="&tea;ASTASpiceFlavor"/>
        <rdfs:subClassOf rdf:resource="&tea;SpicyFlavor"/>
        <skos:definition>a flavor listed in the ASTA list that is reminiscent of star anise, the fruit of the tree Illicium verum</skos:definition>
        <dct:source>ASTA spice list (http://www.astaspice.org/download/9423/)</dct:source>
    </owl:Class>
    


    <!-- http://tw.rpi.edu/web/Courses/Ontologies/2016/OE_9_TeaTeam/SteepedDrink -->

    <owl:Class rdf:about="&tea;SteepedDrink">
        <rdfs:label xml:lang="en">steeped drink</rdfs:label>
        <owl:equivalentClass>
            <owl:Restriction>
                <owl:onProperty rdf:resource="&tea;hasFlavor"/>
                <owl:onClass rdf:resource="&tea;Flavor"/>
                <owl:minQualifiedCardinality rdf:datatype="&xsd;nonNegativeInteger">1</owl:minQualifiedCardinality>
            </owl:Restriction>
        </owl:equivalentClass>
        <owl:equivalentClass>
            <owl:Restriction>
                <owl:onProperty rdf:resource="&tea;hasBrewingTemperature"/>
                <owl:onClass rdf:resource="&tea;BrewingTemperature"/>
                <owl:minQualifiedCardinality rdf:datatype="&xsd;nonNegativeInteger">1</owl:minQualifiedCardinality>
            </owl:Restriction>
        </owl:equivalentClass>
        <rdfs:subClassOf rdf:resource="&tea;DomainConcept"/>
        <dct:source>Adapted from Merriam-Webster: http://www.merriam-webster.com/dictionary/steep (sense 3)</dct:source>
        <skos:definition xml:lang="en">A beverage that has been prepared by allowing ingredients to soak in water at a temperature under the boiling point.</skos:definition>
    </owl:Class>
    


    <!-- http://tw.rpi.edu/web/Courses/Ontologies/2016/OE_9_TeaTeam/SweetFlavor -->

    <owl:Class rdf:about="&tea;SweetFlavor">
        <rdfs:label xml:lang="en">sweet flavor</rdfs:label>
        <rdfs:subClassOf rdf:resource="&tea;Flavor"/>
        <dct:source>Adapted from Tea Cupping Standards (http://www.worldoftea.org/tea-cupping-standards/), Stone Leaf Tea&apos;s Tea Guru (http://www.stoneleaftea.com/tea-guru/), and The Australian Tea Maters&apos; Tea Flavour Wheel (https://australianteamasters.wordpress.com/2014/04/30/the-tea-flavour-wheel/)</dct:source>
        <skos:definition xml:lang="en">a flavor that is sugary or syrupy</skos:definition>
    </owl:Class>
    


    <!-- http://tw.rpi.edu/web/Courses/Ontologies/2016/OE_9_TeaTeam/TarragonFlavor -->

    <owl:Class rdf:about="&tea;TarragonFlavor">
        <rdfs:label xml:lang="en">tarragon flavor</rdfs:label>
        <rdfs:subClassOf rdf:resource="&tea;ASTASpiceFlavor"/>
        <rdfs:subClassOf rdf:resource="&tea;HerbalFlavor"/>
        <skos:definition>a flavor listed in the ASTA list that is reminiscent of tarragon, the leaves of the herb Artemisia dracunculus</skos:definition>
        <dct:source>ASTA spice list (http://www.astaspice.org/download/9423/)</dct:source>
    </owl:Class>
    


    <!-- http://tw.rpi.edu/web/Courses/Ontologies/2016/OE_9_TeaTeam/Tea -->

    <owl:Class rdf:about="&tea;Tea">
        <rdfs:label xml:lang="en">tea</rdfs:label>
        <rdfs:subClassOf rdf:resource="&tea;CaffeinatedSteepedDrink"/>
        <skos:altLabel>茶</skos:altLabel>
        <dct:source>Tea: The Drink that Changed the World</dct:source>
        <skos:definition>A steeped drink made from the leaves of the Camellia sinensis plant</skos:definition>
    </owl:Class>
    


    <!-- http://tw.rpi.edu/web/Courses/Ontologies/2016/OE_9_TeaTeam/ThymeFlavor -->

    <owl:Class rdf:about="&tea;ThymeFlavor">
        <rdfs:label xml:lang="en">thyme flavor</rdfs:label>
        <rdfs:subClassOf rdf:resource="&tea;ASTASpiceFlavor"/>
        <rdfs:subClassOf rdf:resource="&tea;HerbalFlavor"/>
        <dct:source>ASTA spice list (http://www.astaspice.org/download/9423/)</dct:source>
        <skos:definition>a flavor listed in the ASTA list that is reminiscent of thyme, the leaves of the plant Thymus vulgaris</skos:definition>
    </owl:Class>
    


    <!-- http://tw.rpi.edu/web/Courses/Ontologies/2016/OE_9_TeaTeam/Tisane -->

    <owl:Class rdf:about="&tea;Tisane">
        <rdfs:label xml:lang="en">tisane</rdfs:label>
        <rdfs:subClassOf rdf:resource="&tea;SteepedDrink"/>
        <dct:source>Tea: The Drink that Changed the World</dct:source>
        <skos:definition>A steeped drink made from plants other than Camellia sinensis</skos:definition>
        <skos:altLabel xml:lang="en">herbal tea</skos:altLabel>
    </owl:Class>
    


    <!-- http://tw.rpi.edu/web/Courses/Ontologies/2016/OE_9_TeaTeam/ValuePartition -->

    <owl:Class rdf:about="&tea;ValuePartition">
        <rdfs:label xml:lang="en">value partition</rdfs:label>
    </owl:Class>
    


    <!-- http://tw.rpi.edu/web/Courses/Ontologies/2016/OE_9_TeaTeam/VanillaFlavor -->

    <owl:Class rdf:about="&tea;VanillaFlavor">
        <rdfs:label xml:lang="en">vanilla flavor</rdfs:label>
        <rdfs:subClassOf rdf:resource="&tea;ASTASpiceFlavor"/>
        <rdfs:subClassOf rdf:resource="&tea;SweetFlavor"/>
        <skos:definition>a flavor listed in the ASTA list that is reminiscent of vanilla, the seed pods of flowering vines in the genus Vanilla, typically Vanilla planifolia</skos:definition>
        <dct:source>ASTA spice list (http://www.astaspice.org/download/9423/)</dct:source>
    </owl:Class>
    


    <!-- http://tw.rpi.edu/web/Courses/Ontologies/2016/OE_9_TeaTeam/VegetalFlavor -->

    <owl:Class rdf:about="&tea;VegetalFlavor">
        <rdfs:label xml:lang="en">vegetal flavor</rdfs:label>
        <rdfs:subClassOf rdf:resource="&tea;Flavor"/>
        <dct:source>Adapted from Tea Cupping Standards (http://www.worldoftea.org/tea-cupping-standards/), Stone Leaf Tea&apos;s Tea Guru (http://www.stoneleaftea.com/tea-guru/), and The Australian Tea Maters&apos; Tea Flavour Wheel (https://australianteamasters.wordpress.com/2014/04/30/the-tea-flavour-wheel/)</dct:source>
        <skos:definition xml:lang="en">a flavor that is leafy, grassy, or evocative of a vegetable</skos:definition>
    </owl:Class>
    


    <!-- http://tw.rpi.edu/web/Courses/Ontologies/2016/OE_9_TeaTeam/WhitePepperFlavor -->

    <owl:Class rdf:about="&tea;WhitePepperFlavor">
        <rdfs:label xml:lang="en">white pepper flavor</rdfs:label>
        <rdfs:subClassOf rdf:resource="&tea;ASTASpiceFlavor"/>
        <rdfs:subClassOf rdf:resource="&tea;SpicyFlavor"/>
        <skos:definition>a flavor listed in the ASTA list that is reminiscent of white pepper, the seeds of the plant Piper nigrum that has had the skin of the fruit removed</skos:definition>
        <dct:source>ASTA spice list (http://www.astaspice.org/download/9423/)</dct:source>
    </owl:Class>
    


    <!-- http://tw.rpi.edu/web/Courses/Ontologies/2016/OE_9_TeaTeam/WhiteTea -->

    <owl:Class rdf:about="&tea;WhiteTea">
        <rdfs:label xml:lang="en">white tea</rdfs:label>
        <rdfs:subClassOf rdf:resource="&tea;Tea"/>
        <skos:altLabel>白茶</skos:altLabel>
        <dct:source>Tea: The Drink that Changed the World</dct:source>
        <skos:definition>Tea that has been dried, but not withered, rolled, or oxidized</skos:definition>
    </owl:Class>
    


    <!-- http://tw.rpi.edu/web/Courses/Ontologies/2016/OE_9_TeaTeam/WoodyFlavor -->

    <owl:Class rdf:about="&tea;WoodyFlavor">
        <rdfs:label xml:lang="en">woody flavor</rdfs:label>
        <rdfs:subClassOf rdf:resource="&tea;Flavor"/>
        <dct:source>Adapted from Tea Cupping Standards (http://www.worldoftea.org/tea-cupping-standards/), Stone Leaf Tea&apos;s Tea Guru (http://www.stoneleaftea.com/tea-guru/), and The Australian Tea Maters&apos; Tea Flavour Wheel (https://australianteamasters.wordpress.com/2014/04/30/the-tea-flavour-wheel/)</dct:source>
        <skos:definition xml:lang="en">a flavor that is evocative of wood or trees</skos:definition>
    </owl:Class>
    


    <!-- http://tw.rpi.edu/web/Courses/Ontologies/2016/OE_9_TeaTeam/YerbaMate -->

    <owl:Class rdf:about="&tea;YerbaMate">
        <rdfs:label xml:lang="en">yerba mate</rdfs:label>
        <rdfs:subClassOf rdf:resource="&tea;CaffeinatedSteepedDrink"/>
        <rdfs:subClassOf rdf:resource="&tea;Tisane"/>
        <skos:definition>A steeped drink made from the leaves of Ilex paraguariensis, grown in South America. Contains caffeine.</skos:definition>
        <dct:source>Tea: The Drink that Changed the World</dct:source>
    </owl:Class>
    


    <!-- http://tw.rpi.edu/web/Courses/Ontologies/2016/OE_9_TeaTeam/YoungRawPu-ErhTea -->

    <owl:Class rdf:about="&tea;YoungRawPu-ErhTea">
        <rdfs:label xml:lang="en">young raw pu-erh tea</rdfs:label>
        <rdfs:subClassOf rdf:resource="&tea;Pu-ErhTea"/>
        <rdfs:subClassOf>
            <owl:Restriction>
                <owl:onProperty rdf:resource="&tea;hasBrewingTemperature"/>
                <owl:someValuesFrom rdf:resource="&tea;MediumBrewingTemperature"/>
            </owl:Restriction>
        </rdfs:subClassOf>
        <skos:definition>A pu-erh tea that is less than three years old</skos:definition>
        <dct:source>http://www.seriouseats.com/2015/08/what-is-puerh-tea-where-to-buy.html</dct:source>
    </owl:Class>
    


    <!-- http://www.nanopub.org/nschema#Assertion -->

    <owl:Class rdf:about="&np;Assertion">
        <rdfs:label xml:lang="en">Assertion</rdfs:label>
        <rdfs:subClassOf rdf:resource="&rdfg-1;Graph"/>
    </owl:Class>
    


    <!-- http://www.nanopub.org/nschema#Nanopublication -->

    <owl:Class rdf:about="&np;Nanopublication">
        <rdfs:label xml:lang="en">Nanopublication</rdfs:label>
    </owl:Class>
    


    <!-- http://www.w3.org/2004/03/trix/rdfg-1/Graph -->

    <owl:Class rdf:about="&rdfg-1;Graph"/>
</rdf:RDF>



<!-- Generated by the OWL API (version 3.4.2) http://owlapi.sourceforge.net -->

